powerpc/ConstpropOp.v
@@ -32,9 +32,10 @@ Inductive approx : Type :=
                              no compile-time information is available. *)
   | I: int -> approx     (** A known integer value. *)
   | F: float -> approx   (** A known floating-point value. *)
-  | S: ident -> int -> approx.
+  | G: ident -> int -> approx
                          (** The value is the address of the given global
                              symbol plus the given integer offset. *)
+  | S: int -> approx.    (** The value is the stack pointer plus the offset. *)
 
 (** We now define the abstract interpretations of conditions and operators
   over this set of approximations.  For instance, the abstract interpretation
@@ -47,8 +48,9 @@ Inductive approx : Type :=
   indirect style described in file [Cmconstr] to avoid excessive
   duplication of cases in proofs. *)
 
-(*
-Definition eval_static_condition (cond: condition) (vl: list approx) :=
+(** Original definition:
+<<
+Nondetfunction eval_static_condition (cond: condition) (vl: list approx) :=
   match cond, vl with
   | Ccomp c, I n1 :: I n2 :: nil => Some(Int.cmp c n1 n2)
   | Ccompu c, I n1 :: I n2 :: nil => Some(Int.cmpu c n1 n2)
@@ -57,101 +59,90 @@ Definition eval_static_condition (cond: condition) (vl: list approx) :=
   | Ccompf c, F n1 :: F n2 :: nil => Some(Float.cmp c n1 n2)
   | Cnotcompf c, F n1 :: F n2 :: nil => Some(negb(Float.cmp c n1 n2))
   | Cmaskzero n, I n1 :: nil => Some(Int.eq (Int.and n1 n) Int.zero)
-  | Cmasknotzero n, n1::nil => Some(negb(Int.eq (Int.and n1 n) Int.zero))
+  | Cmasknotzero n, I n1::nil => Some(negb(Int.eq (Int.and n1 n) Int.zero))
   | _, _ => None
   end.
+>>
 *)
 
 Inductive eval_static_condition_cases: forall (cond: condition) (vl: list approx), Type :=
-  | eval_static_condition_case1:
-      forall c n1 n2,
-      eval_static_condition_cases (Ccomp c) (I n1 :: I n2 :: nil)
-  | eval_static_condition_case2:
-      forall c n1 n2,
-      eval_static_condition_cases (Ccompu c) (I n1 :: I n2 :: nil)
-  | eval_static_condition_case3:
-      forall c n n1,
-      eval_static_condition_cases (Ccompimm c n) (I n1 :: nil)
-  | eval_static_condition_case4:
-      forall c n n1,
-      eval_static_condition_cases (Ccompuimm c n) (I n1 :: nil)
-  | eval_static_condition_case5:
-      forall c n1 n2,
-      eval_static_condition_cases (Ccompf c) (F n1 :: F n2 :: nil)
-  | eval_static_condition_case6:
-      forall c n1 n2,
-      eval_static_condition_cases (Cnotcompf c) (F n1 :: F n2 :: nil)
-  | eval_static_condition_case7:
-      forall n n1,
-      eval_static_condition_cases (Cmaskzero n) (I n1 :: nil)
-  | eval_static_condition_case8:
-      forall n n1,
-      eval_static_condition_cases (Cmasknotzero n) (I n1 :: nil)
-  | eval_static_condition_default:
-      forall (cond: condition) (vl: list approx),
-      eval_static_condition_cases cond vl.
+  | eval_static_condition_case1: forall c n1 n2, eval_static_condition_cases (Ccomp c) (I n1 :: I n2 :: nil)
+  | eval_static_condition_case2: forall c n1 n2, eval_static_condition_cases (Ccompu c) (I n1 :: I n2 :: nil)
+  | eval_static_condition_case3: forall c n n1, eval_static_condition_cases (Ccompimm c n) (I n1 :: nil)
+  | eval_static_condition_case4: forall c n n1, eval_static_condition_cases (Ccompuimm c n) (I n1 :: nil)
+  | eval_static_condition_case5: forall c n1 n2, eval_static_condition_cases (Ccompf c) (F n1 :: F n2 :: nil)
+  | eval_static_condition_case6: forall c n1 n2, eval_static_condition_cases (Cnotcompf c) (F n1 :: F n2 :: nil)
+  | eval_static_condition_case7: forall n n1, eval_static_condition_cases (Cmaskzero n) (I n1 :: nil)
+  | eval_static_condition_case8: forall n n1, eval_static_condition_cases (Cmasknotzero n) (I n1::nil)
+  | eval_static_condition_default: forall (cond: condition) (vl: list approx), eval_static_condition_cases cond vl.
 
 Definition eval_static_condition_match (cond: condition) (vl: list approx) :=
-  match cond as z1, vl as z2 return eval_static_condition_cases z1 z2 with
-  | Ccomp c, I n1 :: I n2 :: nil =>
-      eval_static_condition_case1 c n1 n2
-  | Ccompu c, I n1 :: I n2 :: nil =>
-      eval_static_condition_case2 c n1 n2
-  | Ccompimm c n, I n1 :: nil =>
-      eval_static_condition_case3 c n n1
-  | Ccompuimm c n, I n1 :: nil =>
-      eval_static_condition_case4 c n n1
-  | Ccompf c, F n1 :: F n2 :: nil =>
-      eval_static_condition_case5 c n1 n2
-  | Cnotcompf c, F n1 :: F n2 :: nil =>
-      eval_static_condition_case6 c n1 n2
-  | Cmaskzero n, I n1 :: nil =>
-      eval_static_condition_case7 n n1
-  | Cmasknotzero n, I n1 :: nil =>
-      eval_static_condition_case8 n n1
-  | cond, vl =>
-      eval_static_condition_default cond vl
+  match cond as zz1, vl as zz2 return eval_static_condition_cases zz1 zz2 with
+  | Ccomp c, I n1 :: I n2 :: nil => eval_static_condition_case1 c n1 n2
+  | Ccompu c, I n1 :: I n2 :: nil => eval_static_condition_case2 c n1 n2
+  | Ccompimm c n, I n1 :: nil => eval_static_condition_case3 c n n1
+  | Ccompuimm c n, I n1 :: nil => eval_static_condition_case4 c n n1
+  | Ccompf c, F n1 :: F n2 :: nil => eval_static_condition_case5 c n1 n2
+  | Cnotcompf c, F n1 :: F n2 :: nil => eval_static_condition_case6 c n1 n2
+  | Cmaskzero n, I n1 :: nil => eval_static_condition_case7 n n1
+  | Cmasknotzero n, I n1::nil => eval_static_condition_case8 n n1
+  | cond, vl => eval_static_condition_default cond vl
   end.
 
 Definition eval_static_condition (cond: condition) (vl: list approx) :=
   match eval_static_condition_match cond vl with
-  | eval_static_condition_case1 c n1 n2 =>
+  | eval_static_condition_case1 c n1 n2 => (* Ccomp c, I n1 :: I n2 :: nil *) 
       Some(Int.cmp c n1 n2)
-  | eval_static_condition_case2 c n1 n2 =>
+  | eval_static_condition_case2 c n1 n2 => (* Ccompu c, I n1 :: I n2 :: nil *) 
       Some(Int.cmpu c n1 n2)
-  | eval_static_condition_case3 c n n1 =>
+  | eval_static_condition_case3 c n n1 => (* Ccompimm c n, I n1 :: nil *) 
       Some(Int.cmp c n1 n)
-  | eval_static_condition_case4 c n n1 =>
+  | eval_static_condition_case4 c n n1 => (* Ccompuimm c n, I n1 :: nil *) 
       Some(Int.cmpu c n1 n)
-  | eval_static_condition_case5 c n1 n2 =>
+  | eval_static_condition_case5 c n1 n2 => (* Ccompf c, F n1 :: F n2 :: nil *) 
       Some(Float.cmp c n1 n2)
-  | eval_static_condition_case6 c n1 n2 =>
+  | eval_static_condition_case6 c n1 n2 => (* Cnotcompf c, F n1 :: F n2 :: nil *) 
       Some(negb(Float.cmp c n1 n2))
-  | eval_static_condition_case7 n n1 =>
+  | eval_static_condition_case7 n n1 => (* Cmaskzero n, I n1 :: nil *) 
       Some(Int.eq (Int.and n1 n) Int.zero)
-  | eval_static_condition_case8 n n1 =>
+  | eval_static_condition_case8 n n1 => (* Cmasknotzero n, I n1::nil *) 
       Some(negb(Int.eq (Int.and n1 n) Int.zero))
   | eval_static_condition_default cond vl =>
       None
   end.
 
-(*
-Definition eval_static_operation (op: operation) (vl: list approx) :=
+
+Definition eval_static_condition_val (cond: condition) (vl: list approx) :=
+  match eval_static_condition cond vl with
+  | None => Unknown
+  | Some b => I(if b then Int.one else Int.zero)
+  end.
+
+Definition eval_static_intoffloat (f: float) :=
+  match Float.intoffloat f with Some x => I x | None => Unknown end.
+
+(** Original definition:
+<<
+Nondetfunction eval_static_operation (op: operation) (vl: list approx) :=
   match op, vl with
   | Omove, v1::nil => v1
   | Ointconst n, nil => I n
   | Ofloatconst n, nil => F n
-  | Oaddrsymbol s n, nil => S s n
-  | Ocast8signed, I n1 :: nil => I(Int.sign_ext 8 n)
-  | Ocast8unsigned, I n1 :: nil => I(Int.zero_ext 8 n)
-  | Ocast16signed, I n1 :: nil => I(Int.sign_ext 16 n)
-  | Ocast16unsigned, I n1 :: nil => I(Int.zero_ext 16 n)
+  | Oaddrsymbol s n, nil => G s n
+  | Oaddrstack n, nil => S n
+  | Ocast8signed, I n1 :: nil => I(Int.sign_ext 8 n1)
+  | Ocast16signed, I n1 :: nil => I(Int.sign_ext 16 n1)
   | Oadd, I n1 :: I n2 :: nil => I(Int.add n1 n2)
-  | Oadd, S s1 n1 :: I n2 :: nil => S s1 (Int.add n1 n2)
+  | Oadd, G s1 n1 :: I n2 :: nil => G s1 (Int.add n1 n2)
+  | Oadd, I n1 :: G s2 n2 :: nil => G s2 (Int.add n1 n2)
+  | Oadd, S n1 :: I n2 :: nil => S (Int.add n1 n2)
+  | Oadd, I n1 :: S n2 :: nil => S (Int.add n1 n2)
   | Oaddimm n, I n1 :: nil => I (Int.add n1 n)
-  | Oaddimm n, S s1 n1 :: nil => S s1 (Int.add n1 n)
+  | Oaddimm n, G s1 n1 :: nil => G s1 (Int.add n1 n)
+  | Oaddimm n, S n1 :: nil => S (Int.add n1 n)
   | Osub, I n1 :: I n2 :: nil => I(Int.sub n1 n2)
-  | Osub, S s1 n1 :: I n2 :: nil => S s1 (Int.sub n1 n2)
+  | Osub, G s1 n1 :: I n2 :: nil => G s1 (Int.sub n1 n2)
+  | Osub, S n1 :: I n2 :: nil => S (Int.sub n1 n2)
   | Osubimm n, I n1 :: nil => I (Int.sub n n1)
   | Omul, I n1 :: I n2 :: nil => I(Int.mul n1 n2)
   | Omulimm n, I n1 :: nil => I(Int.mul n1 n)
@@ -172,6 +163,7 @@ Definition eval_static_operation (op: operation) (vl: list approx) :=
   | Oshrximm n, I n1 :: nil => if Int.ltu n Int.iwordsize then I(Int.shrx n1 n) else Unknown
   | Oshru, I n1 :: I n2 :: nil => if Int.ltu n2 Int.iwordsize then I(Int.shru n1 n2) else Unknown
   | Orolm amount mask, I n1 :: nil => I(Int.rolm n1 amount mask)
+  | Oroli amount mask, I n1 :: I n2 :: nil => I(Int.or (Int.and n1 (Int.not mask)) (Int.rolm n2 amount mask))
   | Onegf, F n1 :: nil => F(Float.neg n1)
   | Oabsf, F n1 :: nil => F(Float.abs n1)
   | Oaddf, F n1 :: F n2 :: nil => F(Float.add n1 n2)
@@ -181,358 +173,232 @@ Definition eval_static_operation (op: operation) (vl: list approx) :=
   | Omuladdf, F n1 :: F n2 :: F n3 :: nil => F(Float.add (Float.mul n1 n2) n3)
   | Omulsubf, F n1 :: F n2 :: F n3 :: nil => F(Float.sub (Float.mul n1 n2) n3)
   | Osingleoffloat, F n1 :: nil => F(Float.singleoffloat n1)
-  | Ointoffloat, F n1 :: nil => match Float.intoffloat n1 with Some x => I x | None => Unknown end
+  | Ointoffloat, F n1 :: nil => eval_static_intoffloat n1
   | Ofloatofwords, I n1 :: I n2 :: nil => F(Float.from_words n1 n2)
-  | Ocmp c, vl =>
-      match eval_static_condition c vl with
-      | None => Unknown
-      | Some b => I(if b then Int.one else Int.zero)
-      end
+  | Ocmp c, vl => eval_static_condition_val c vl
   | _, _ => Unknown
   end.
+>>
 *)
 
 Inductive eval_static_operation_cases: forall (op: operation) (vl: list approx), Type :=
-  | eval_static_operation_case1:
-      forall v1,
-      eval_static_operation_cases (Omove) (v1::nil)
-  | eval_static_operation_case2:
-      forall n,
-      eval_static_operation_cases (Ointconst n) (nil)
-  | eval_static_operation_case3:
-      forall n,
-      eval_static_operation_cases (Ofloatconst n) (nil)
-  | eval_static_operation_case4:
-      forall s n,
-      eval_static_operation_cases (Oaddrsymbol s n) (nil)
-  | eval_static_operation_case6:
-      forall n1,
-      eval_static_operation_cases (Ocast8signed) (I n1 :: nil)
-  | eval_static_operation_case7:
-      forall n1,
-      eval_static_operation_cases (Ocast16signed) (I n1 :: nil)
-  | eval_static_operation_case8:
-      forall n1 n2,
-      eval_static_operation_cases (Oadd) (I n1 :: I n2 :: nil)
-  | eval_static_operation_case9:
-      forall s1 n1 n2,
-      eval_static_operation_cases (Oadd) (S s1 n1 :: I n2 :: nil)
-  | eval_static_operation_case11:
-      forall n n1,
-      eval_static_operation_cases (Oaddimm n) (I n1 :: nil)
-  | eval_static_operation_case12:
-      forall n s1 n1,
-      eval_static_operation_cases (Oaddimm n) (S s1 n1 :: nil)
-  | eval_static_operation_case13:
-      forall n1 n2,
-      eval_static_operation_cases (Osub) (I n1 :: I n2 :: nil)
-  | eval_static_operation_case14:
-      forall s1 n1 n2,
-      eval_static_operation_cases (Osub) (S s1 n1 :: I n2 :: nil)
-  | eval_static_operation_case15:
-      forall n n1,
-      eval_static_operation_cases (Osubimm n) (I n1 :: nil)
-  | eval_static_operation_case16:
-      forall n1 n2,
-      eval_static_operation_cases (Omul) (I n1 :: I n2 :: nil)
-  | eval_static_operation_case17:
-      forall n n1,
-      eval_static_operation_cases (Omulimm n) (I n1 :: nil)
-  | eval_static_operation_case18:
-      forall n1 n2,
-      eval_static_operation_cases (Odiv) (I n1 :: I n2 :: nil)
-  | eval_static_operation_case19:
-      forall n1 n2,
-      eval_static_operation_cases (Odivu) (I n1 :: I n2 :: nil)
-  | eval_static_operation_case20:
-      forall n1 n2,
-      eval_static_operation_cases (Oand) (I n1 :: I n2 :: nil)
-  | eval_static_operation_case21:
-      forall n n1,
-      eval_static_operation_cases (Oandimm n) (I n1 :: nil)
-  | eval_static_operation_case22:
-      forall n1 n2,
-      eval_static_operation_cases (Oor) (I n1 :: I n2 :: nil)
-  | eval_static_operation_case23:
-      forall n n1,
-      eval_static_operation_cases (Oorimm n) (I n1 :: nil)
-  | eval_static_operation_case24:
-      forall n1 n2,
-      eval_static_operation_cases (Oxor) (I n1 :: I n2 :: nil)
-  | eval_static_operation_case25:
-      forall n n1,
-      eval_static_operation_cases (Oxorimm n) (I n1 :: nil)
-  | eval_static_operation_case26:
-      forall n1 n2,
-      eval_static_operation_cases (Onand) (I n1 :: I n2 :: nil)
-  | eval_static_operation_case27:
-      forall n1 n2,
-      eval_static_operation_cases (Onor) (I n1 :: I n2 :: nil)
-  | eval_static_operation_case28:
-      forall n1 n2,
-      eval_static_operation_cases (Onxor) (I n1 :: I n2 :: nil)
-  | eval_static_operation_case29:
-      forall n1 n2,
-      eval_static_operation_cases (Oshl) (I n1 :: I n2 :: nil)
-  | eval_static_operation_case30:
-      forall n1 n2,
-      eval_static_operation_cases (Oshr) (I n1 :: I n2 :: nil)
-  | eval_static_operation_case31:
-      forall n n1,
-      eval_static_operation_cases (Oshrimm n) (I n1 :: nil)
-  | eval_static_operation_case32:
-      forall n n1,
-      eval_static_operation_cases (Oshrximm n) (I n1 :: nil)
-  | eval_static_operation_case33:
-      forall n1 n2,
-      eval_static_operation_cases (Oshru) (I n1 :: I n2 :: nil)
-  | eval_static_operation_case34:
-      forall amount mask n1,
-      eval_static_operation_cases (Orolm amount mask) (I n1 :: nil)
-  | eval_static_operation_case35:
-      forall n1,
-      eval_static_operation_cases (Onegf) (F n1 :: nil)
-  | eval_static_operation_case36:
-      forall n1,
-      eval_static_operation_cases (Oabsf) (F n1 :: nil)
-  | eval_static_operation_case37:
-      forall n1 n2,
-      eval_static_operation_cases (Oaddf) (F n1 :: F n2 :: nil)
-  | eval_static_operation_case38:
-      forall n1 n2,
-      eval_static_operation_cases (Osubf) (F n1 :: F n2 :: nil)
-  | eval_static_operation_case39:
-      forall n1 n2,
-      eval_static_operation_cases (Omulf) (F n1 :: F n2 :: nil)
-  | eval_static_operation_case40:
-      forall n1 n2,
-      eval_static_operation_cases (Odivf) (F n1 :: F n2 :: nil)
-  | eval_static_operation_case41:
-      forall n1 n2 n3,
-      eval_static_operation_cases (Omuladdf) (F n1 :: F n2 :: F n3 :: nil)
-  | eval_static_operation_case42:
-      forall n1 n2 n3,
-      eval_static_operation_cases (Omulsubf) (F n1 :: F n2 :: F n3 :: nil)
-  | eval_static_operation_case43:
-      forall n1,
-      eval_static_operation_cases (Osingleoffloat) (F n1 :: nil)
-  | eval_static_operation_case44:
-      forall n1,
-      eval_static_operation_cases (Ointoffloat) (F n1 :: nil)
-  | eval_static_operation_case45:
-      forall n1 n2,
-      eval_static_operation_cases (Ofloatofwords) (I n1 :: I n2 :: nil)
-  | eval_static_operation_case47:
-      forall c vl,
-      eval_static_operation_cases (Ocmp c) (vl)
-  | eval_static_operation_case48:
-      forall n1,
-      eval_static_operation_cases (Ocast8unsigned) (I n1 :: nil)
-  | eval_static_operation_case49:
-      forall n1,
-      eval_static_operation_cases (Ocast16unsigned) (I n1 :: nil)
-  | eval_static_operation_default:
-      forall (op: operation) (vl: list approx),
-      eval_static_operation_cases op vl.
+  | eval_static_operation_case1: forall v1, eval_static_operation_cases (Omove) (v1::nil)
+  | eval_static_operation_case2: forall n, eval_static_operation_cases (Ointconst n) (nil)
+  | eval_static_operation_case3: forall n, eval_static_operation_cases (Ofloatconst n) (nil)
+  | eval_static_operation_case4: forall s n, eval_static_operation_cases (Oaddrsymbol s n) (nil)
+  | eval_static_operation_case5: forall n, eval_static_operation_cases (Oaddrstack n) (nil)
+  | eval_static_operation_case6: forall n1, eval_static_operation_cases (Ocast8signed) (I n1 :: nil)
+  | eval_static_operation_case7: forall n1, eval_static_operation_cases (Ocast16signed) (I n1 :: nil)
+  | eval_static_operation_case8: forall n1 n2, eval_static_operation_cases (Oadd) (I n1 :: I n2 :: nil)
+  | eval_static_operation_case9: forall s1 n1 n2, eval_static_operation_cases (Oadd) (G s1 n1 :: I n2 :: nil)
+  | eval_static_operation_case10: forall n1 s2 n2, eval_static_operation_cases (Oadd) (I n1 :: G s2 n2 :: nil)
+  | eval_static_operation_case11: forall n1 n2, eval_static_operation_cases (Oadd) (S n1 :: I n2 :: nil)
+  | eval_static_operation_case12: forall n1 n2, eval_static_operation_cases (Oadd) (I n1 :: S n2 :: nil)
+  | eval_static_operation_case13: forall n n1, eval_static_operation_cases (Oaddimm n) (I n1 :: nil)
+  | eval_static_operation_case14: forall n s1 n1, eval_static_operation_cases (Oaddimm n) (G s1 n1 :: nil)
+  | eval_static_operation_case15: forall n n1, eval_static_operation_cases (Oaddimm n) (S n1 :: nil)
+  | eval_static_operation_case16: forall n1 n2, eval_static_operation_cases (Osub) (I n1 :: I n2 :: nil)
+  | eval_static_operation_case17: forall s1 n1 n2, eval_static_operation_cases (Osub) (G s1 n1 :: I n2 :: nil)
+  | eval_static_operation_case18: forall n1 n2, eval_static_operation_cases (Osub) (S n1 :: I n2 :: nil)
+  | eval_static_operation_case19: forall n n1, eval_static_operation_cases (Osubimm n) (I n1 :: nil)
+  | eval_static_operation_case20: forall n1 n2, eval_static_operation_cases (Omul) (I n1 :: I n2 :: nil)
+  | eval_static_operation_case21: forall n n1, eval_static_operation_cases (Omulimm n) (I n1 :: nil)
+  | eval_static_operation_case22: forall n1 n2, eval_static_operation_cases (Odiv) (I n1 :: I n2 :: nil)
+  | eval_static_operation_case23: forall n1 n2, eval_static_operation_cases (Odivu) (I n1 :: I n2 :: nil)
+  | eval_static_operation_case24: forall n1 n2, eval_static_operation_cases (Oand) (I n1 :: I n2 :: nil)
+  | eval_static_operation_case25: forall n n1, eval_static_operation_cases (Oandimm n) (I n1 :: nil)
+  | eval_static_operation_case26: forall n1 n2, eval_static_operation_cases (Oor) (I n1 :: I n2 :: nil)
+  | eval_static_operation_case27: forall n n1, eval_static_operation_cases (Oorimm n) (I n1 :: nil)
+  | eval_static_operation_case28: forall n1 n2, eval_static_operation_cases (Oxor) (I n1 :: I n2 :: nil)
+  | eval_static_operation_case29: forall n n1, eval_static_operation_cases (Oxorimm n) (I n1 :: nil)
+  | eval_static_operation_case30: forall n1 n2, eval_static_operation_cases (Onand) (I n1 :: I n2 :: nil)
+  | eval_static_operation_case31: forall n1 n2, eval_static_operation_cases (Onor) (I n1 :: I n2 :: nil)
+  | eval_static_operation_case32: forall n1 n2, eval_static_operation_cases (Onxor) (I n1 :: I n2 :: nil)
+  | eval_static_operation_case33: forall n1 n2, eval_static_operation_cases (Oshl) (I n1 :: I n2 :: nil)
+  | eval_static_operation_case34: forall n1 n2, eval_static_operation_cases (Oshr) (I n1 :: I n2 :: nil)
+  | eval_static_operation_case35: forall n n1, eval_static_operation_cases (Oshrimm n) (I n1 :: nil)
+  | eval_static_operation_case36: forall n n1, eval_static_operation_cases (Oshrximm n) (I n1 :: nil)
+  | eval_static_operation_case37: forall n1 n2, eval_static_operation_cases (Oshru) (I n1 :: I n2 :: nil)
+  | eval_static_operation_case38: forall amount mask n1, eval_static_operation_cases (Orolm amount mask) (I n1 :: nil)
+  | eval_static_operation_case39: forall amount mask n1 n2, eval_static_operation_cases (Oroli amount mask) (I n1 :: I n2 :: nil)
+  | eval_static_operation_case40: forall n1, eval_static_operation_cases (Onegf) (F n1 :: nil)
+  | eval_static_operation_case41: forall n1, eval_static_operation_cases (Oabsf) (F n1 :: nil)
+  | eval_static_operation_case42: forall n1 n2, eval_static_operation_cases (Oaddf) (F n1 :: F n2 :: nil)
+  | eval_static_operation_case43: forall n1 n2, eval_static_operation_cases (Osubf) (F n1 :: F n2 :: nil)
+  | eval_static_operation_case44: forall n1 n2, eval_static_operation_cases (Omulf) (F n1 :: F n2 :: nil)
+  | eval_static_operation_case45: forall n1 n2, eval_static_operation_cases (Odivf) (F n1 :: F n2 :: nil)
+  | eval_static_operation_case46: forall n1 n2 n3, eval_static_operation_cases (Omuladdf) (F n1 :: F n2 :: F n3 :: nil)
+  | eval_static_operation_case47: forall n1 n2 n3, eval_static_operation_cases (Omulsubf) (F n1 :: F n2 :: F n3 :: nil)
+  | eval_static_operation_case48: forall n1, eval_static_operation_cases (Osingleoffloat) (F n1 :: nil)
+  | eval_static_operation_case49: forall n1, eval_static_operation_cases (Ointoffloat) (F n1 :: nil)
+  | eval_static_operation_case50: forall n1 n2, eval_static_operation_cases (Ofloatofwords) (I n1 :: I n2 :: nil)
+  | eval_static_operation_case51: forall c vl, eval_static_operation_cases (Ocmp c) (vl)
+  | eval_static_operation_default: forall (op: operation) (vl: list approx), eval_static_operation_cases op vl.
 
 Definition eval_static_operation_match (op: operation) (vl: list approx) :=
-  match op as z1, vl as z2 return eval_static_operation_cases z1 z2 with
-  | Omove, v1::nil =>
-      eval_static_operation_case1 v1
-  | Ointconst n, nil =>
-      eval_static_operation_case2 n
-  | Ofloatconst n, nil =>
-      eval_static_operation_case3 n
-  | Oaddrsymbol s n, nil =>
-      eval_static_operation_case4 s n
-  | Ocast8signed, I n1 :: nil =>
-      eval_static_operation_case6 n1
-  | Ocast16signed, I n1 :: nil =>
-      eval_static_operation_case7 n1
-  | Oadd, I n1 :: I n2 :: nil =>
-      eval_static_operation_case8 n1 n2
-  | Oadd, S s1 n1 :: I n2 :: nil =>
-      eval_static_operation_case9 s1 n1 n2
-  | Oaddimm n, I n1 :: nil =>
-      eval_static_operation_case11 n n1
-  | Oaddimm n, S s1 n1 :: nil =>
-      eval_static_operation_case12 n s1 n1
-  | Osub, I n1 :: I n2 :: nil =>
-      eval_static_operation_case13 n1 n2
-  | Osub, S s1 n1 :: I n2 :: nil =>
-      eval_static_operation_case14 s1 n1 n2
-  | Osubimm n, I n1 :: nil =>
-      eval_static_operation_case15 n n1
-  | Omul, I n1 :: I n2 :: nil =>
-      eval_static_operation_case16 n1 n2
-  | Omulimm n, I n1 :: nil =>
-      eval_static_operation_case17 n n1
-  | Odiv, I n1 :: I n2 :: nil =>
-      eval_static_operation_case18 n1 n2
-  | Odivu, I n1 :: I n2 :: nil =>
-      eval_static_operation_case19 n1 n2
-  | Oand, I n1 :: I n2 :: nil =>
-      eval_static_operation_case20 n1 n2
-  | Oandimm n, I n1 :: nil =>
-      eval_static_operation_case21 n n1
-  | Oor, I n1 :: I n2 :: nil =>
-      eval_static_operation_case22 n1 n2
-  | Oorimm n, I n1 :: nil =>
-      eval_static_operation_case23 n n1
-  | Oxor, I n1 :: I n2 :: nil =>
-      eval_static_operation_case24 n1 n2
-  | Oxorimm n, I n1 :: nil =>
-      eval_static_operation_case25 n n1
-  | Onand, I n1 :: I n2 :: nil =>
-      eval_static_operation_case26 n1 n2
-  | Onor, I n1 :: I n2 :: nil =>
-      eval_static_operation_case27 n1 n2
-  | Onxor, I n1 :: I n2 :: nil =>
-      eval_static_operation_case28 n1 n2
-  | Oshl, I n1 :: I n2 :: nil =>
-      eval_static_operation_case29 n1 n2
-  | Oshr, I n1 :: I n2 :: nil =>
-      eval_static_operation_case30 n1 n2
-  | Oshrimm n, I n1 :: nil =>
-      eval_static_operation_case31 n n1
-  | Oshrximm n, I n1 :: nil =>
-      eval_static_operation_case32 n n1
-  | Oshru, I n1 :: I n2 :: nil =>
-      eval_static_operation_case33 n1 n2
-  | Orolm amount mask, I n1 :: nil =>
-      eval_static_operation_case34 amount mask n1
-  | Onegf, F n1 :: nil =>
-      eval_static_operation_case35 n1
-  | Oabsf, F n1 :: nil =>
-      eval_static_operation_case36 n1
-  | Oaddf, F n1 :: F n2 :: nil =>
-      eval_static_operation_case37 n1 n2
-  | Osubf, F n1 :: F n2 :: nil =>
-      eval_static_operation_case38 n1 n2
-  | Omulf, F n1 :: F n2 :: nil =>
-      eval_static_operation_case39 n1 n2
-  | Odivf, F n1 :: F n2 :: nil =>
-      eval_static_operation_case40 n1 n2
-  | Omuladdf, F n1 :: F n2 :: F n3 :: nil =>
-      eval_static_operation_case41 n1 n2 n3
-  | Omulsubf, F n1 :: F n2 :: F n3 :: nil =>
-      eval_static_operation_case42 n1 n2 n3
-  | Osingleoffloat, F n1 :: nil =>
-      eval_static_operation_case43 n1
-  | Ointoffloat, F n1 :: nil =>
-      eval_static_operation_case44 n1
-  | Ofloatofwords, I n1 :: I n2 :: nil =>
-      eval_static_operation_case45 n1 n2
-  | Ocmp c, vl =>
-      eval_static_operation_case47 c vl
-  | Ocast8unsigned, I n1 :: nil =>
-      eval_static_operation_case48 n1
-  | Ocast16unsigned, I n1 :: nil =>
-      eval_static_operation_case49 n1
-  | op, vl =>
-      eval_static_operation_default op vl
+  match op as zz1, vl as zz2 return eval_static_operation_cases zz1 zz2 with
+  | Omove, v1::nil => eval_static_operation_case1 v1
+  | Ointconst n, nil => eval_static_operation_case2 n
+  | Ofloatconst n, nil => eval_static_operation_case3 n
+  | Oaddrsymbol s n, nil => eval_static_operation_case4 s n
+  | Oaddrstack n, nil => eval_static_operation_case5 n
+  | Ocast8signed, I n1 :: nil => eval_static_operation_case6 n1
+  | Ocast16signed, I n1 :: nil => eval_static_operation_case7 n1
+  | Oadd, I n1 :: I n2 :: nil => eval_static_operation_case8 n1 n2
+  | Oadd, G s1 n1 :: I n2 :: nil => eval_static_operation_case9 s1 n1 n2
+  | Oadd, I n1 :: G s2 n2 :: nil => eval_static_operation_case10 n1 s2 n2
+  | Oadd, S n1 :: I n2 :: nil => eval_static_operation_case11 n1 n2
+  | Oadd, I n1 :: S n2 :: nil => eval_static_operation_case12 n1 n2
+  | Oaddimm n, I n1 :: nil => eval_static_operation_case13 n n1
+  | Oaddimm n, G s1 n1 :: nil => eval_static_operation_case14 n s1 n1
+  | Oaddimm n, S n1 :: nil => eval_static_operation_case15 n n1
+  | Osub, I n1 :: I n2 :: nil => eval_static_operation_case16 n1 n2
+  | Osub, G s1 n1 :: I n2 :: nil => eval_static_operation_case17 s1 n1 n2
+  | Osub, S n1 :: I n2 :: nil => eval_static_operation_case18 n1 n2
+  | Osubimm n, I n1 :: nil => eval_static_operation_case19 n n1
+  | Omul, I n1 :: I n2 :: nil => eval_static_operation_case20 n1 n2
+  | Omulimm n, I n1 :: nil => eval_static_operation_case21 n n1
+  | Odiv, I n1 :: I n2 :: nil => eval_static_operation_case22 n1 n2
+  | Odivu, I n1 :: I n2 :: nil => eval_static_operation_case23 n1 n2
+  | Oand, I n1 :: I n2 :: nil => eval_static_operation_case24 n1 n2
+  | Oandimm n, I n1 :: nil => eval_static_operation_case25 n n1
+  | Oor, I n1 :: I n2 :: nil => eval_static_operation_case26 n1 n2
+  | Oorimm n, I n1 :: nil => eval_static_operation_case27 n n1
+  | Oxor, I n1 :: I n2 :: nil => eval_static_operation_case28 n1 n2
+  | Oxorimm n, I n1 :: nil => eval_static_operation_case29 n n1
+  | Onand, I n1 :: I n2 :: nil => eval_static_operation_case30 n1 n2
+  | Onor, I n1 :: I n2 :: nil => eval_static_operation_case31 n1 n2
+  | Onxor, I n1 :: I n2 :: nil => eval_static_operation_case32 n1 n2
+  | Oshl, I n1 :: I n2 :: nil => eval_static_operation_case33 n1 n2
+  | Oshr, I n1 :: I n2 :: nil => eval_static_operation_case34 n1 n2
+  | Oshrimm n, I n1 :: nil => eval_static_operation_case35 n n1
+  | Oshrximm n, I n1 :: nil => eval_static_operation_case36 n n1
+  | Oshru, I n1 :: I n2 :: nil => eval_static_operation_case37 n1 n2
+  | Orolm amount mask, I n1 :: nil => eval_static_operation_case38 amount mask n1
+  | Oroli amount mask, I n1 :: I n2 :: nil => eval_static_operation_case39 amount mask n1 n2
+  | Onegf, F n1 :: nil => eval_static_operation_case40 n1
+  | Oabsf, F n1 :: nil => eval_static_operation_case41 n1
+  | Oaddf, F n1 :: F n2 :: nil => eval_static_operation_case42 n1 n2
+  | Osubf, F n1 :: F n2 :: nil => eval_static_operation_case43 n1 n2
+  | Omulf, F n1 :: F n2 :: nil => eval_static_operation_case44 n1 n2
+  | Odivf, F n1 :: F n2 :: nil => eval_static_operation_case45 n1 n2
+  | Omuladdf, F n1 :: F n2 :: F n3 :: nil => eval_static_operation_case46 n1 n2 n3
+  | Omulsubf, F n1 :: F n2 :: F n3 :: nil => eval_static_operation_case47 n1 n2 n3
+  | Osingleoffloat, F n1 :: nil => eval_static_operation_case48 n1
+  | Ointoffloat, F n1 :: nil => eval_static_operation_case49 n1
+  | Ofloatofwords, I n1 :: I n2 :: nil => eval_static_operation_case50 n1 n2
+  | Ocmp c, vl => eval_static_operation_case51 c vl
+  | op, vl => eval_static_operation_default op vl
   end.
 
 Definition eval_static_operation (op: operation) (vl: list approx) :=
   match eval_static_operation_match op vl with
-  | eval_static_operation_case1 v1 =>
+  | eval_static_operation_case1 v1 => (* Omove, v1::nil *) 
       v1
-  | eval_static_operation_case2 n =>
+  | eval_static_operation_case2 n => (* Ointconst n, nil *) 
       I n
-  | eval_static_operation_case3 n =>
+  | eval_static_operation_case3 n => (* Ofloatconst n, nil *) 
       F n
-  | eval_static_operation_case4 s n =>
-      S s n
-  | eval_static_operation_case6 n1 =>
+  | eval_static_operation_case4 s n => (* Oaddrsymbol s n, nil *) 
+      G s n
+  | eval_static_operation_case5 n => (* Oaddrstack n, nil *) 
+      S n
+  | eval_static_operation_case6 n1 => (* Ocast8signed, I n1 :: nil *) 
       I(Int.sign_ext 8 n1)
-  | eval_static_operation_case7 n1 =>
+  | eval_static_operation_case7 n1 => (* Ocast16signed, I n1 :: nil *) 
       I(Int.sign_ext 16 n1)
-  | eval_static_operation_case8 n1 n2 =>
+  | eval_static_operation_case8 n1 n2 => (* Oadd, I n1 :: I n2 :: nil *) 
       I(Int.add n1 n2)
-  | eval_static_operation_case9 s1 n1 n2 =>
-      S s1 (Int.add n1 n2)
-  | eval_static_operation_case11 n n1 =>
+  | eval_static_operation_case9 s1 n1 n2 => (* Oadd, G s1 n1 :: I n2 :: nil *) 
+      G s1 (Int.add n1 n2)
+  | eval_static_operation_case10 n1 s2 n2 => (* Oadd, I n1 :: G s2 n2 :: nil *) 
+      G s2 (Int.add n1 n2)
+  | eval_static_operation_case11 n1 n2 => (* Oadd, S n1 :: I n2 :: nil *) 
+      S (Int.add n1 n2)
+  | eval_static_operation_case12 n1 n2 => (* Oadd, I n1 :: S n2 :: nil *) 
+      S (Int.add n1 n2)
+  | eval_static_operation_case13 n n1 => (* Oaddimm n, I n1 :: nil *) 
       I (Int.add n1 n)
-  | eval_static_operation_case12 n s1 n1 =>
-      S s1 (Int.add n1 n)
-  | eval_static_operation_case13 n1 n2 =>
+  | eval_static_operation_case14 n s1 n1 => (* Oaddimm n, G s1 n1 :: nil *) 
+      G s1 (Int.add n1 n)
+  | eval_static_operation_case15 n n1 => (* Oaddimm n, S n1 :: nil *) 
+      S (Int.add n1 n)
+  | eval_static_operation_case16 n1 n2 => (* Osub, I n1 :: I n2 :: nil *) 
       I(Int.sub n1 n2)
-  | eval_static_operation_case14 s1 n1 n2 =>
-      S s1 (Int.sub n1 n2)
-  | eval_static_operation_case15 n n1 =>
+  | eval_static_operation_case17 s1 n1 n2 => (* Osub, G s1 n1 :: I n2 :: nil *) 
+      G s1 (Int.sub n1 n2)
+  | eval_static_operation_case18 n1 n2 => (* Osub, S n1 :: I n2 :: nil *) 
+      S (Int.sub n1 n2)
+  | eval_static_operation_case19 n n1 => (* Osubimm n, I n1 :: nil *) 
       I (Int.sub n n1)
-  | eval_static_operation_case16 n1 n2 =>
+  | eval_static_operation_case20 n1 n2 => (* Omul, I n1 :: I n2 :: nil *) 
       I(Int.mul n1 n2)
-  | eval_static_operation_case17 n n1 =>
+  | eval_static_operation_case21 n n1 => (* Omulimm n, I n1 :: nil *) 
       I(Int.mul n1 n)
-  | eval_static_operation_case18 n1 n2 =>
+  | eval_static_operation_case22 n1 n2 => (* Odiv, I n1 :: I n2 :: nil *) 
       if Int.eq n2 Int.zero then Unknown else I(Int.divs n1 n2)
-  | eval_static_operation_case19 n1 n2 =>
+  | eval_static_operation_case23 n1 n2 => (* Odivu, I n1 :: I n2 :: nil *) 
       if Int.eq n2 Int.zero then Unknown else I(Int.divu n1 n2)
-  | eval_static_operation_case20 n1 n2 =>
+  | eval_static_operation_case24 n1 n2 => (* Oand, I n1 :: I n2 :: nil *) 
       I(Int.and n1 n2)
-  | eval_static_operation_case21 n n1 =>
+  | eval_static_operation_case25 n n1 => (* Oandimm n, I n1 :: nil *) 
       I(Int.and n1 n)
-  | eval_static_operation_case22 n1 n2 =>
+  | eval_static_operation_case26 n1 n2 => (* Oor, I n1 :: I n2 :: nil *) 
       I(Int.or n1 n2)
-  | eval_static_operation_case23 n n1 =>
+  | eval_static_operation_case27 n n1 => (* Oorimm n, I n1 :: nil *) 
       I(Int.or n1 n)
-  | eval_static_operation_case24 n1 n2 =>
+  | eval_static_operation_case28 n1 n2 => (* Oxor, I n1 :: I n2 :: nil *) 
       I(Int.xor n1 n2)
-  | eval_static_operation_case25 n n1 =>
+  | eval_static_operation_case29 n n1 => (* Oxorimm n, I n1 :: nil *) 
       I(Int.xor n1 n)
-  | eval_static_operation_case26 n1 n2 =>
+  | eval_static_operation_case30 n1 n2 => (* Onand, I n1 :: I n2 :: nil *) 
       I(Int.xor (Int.and n1 n2) Int.mone)
-  | eval_static_operation_case27 n1 n2 =>
+  | eval_static_operation_case31 n1 n2 => (* Onor, I n1 :: I n2 :: nil *) 
       I(Int.xor (Int.or n1 n2) Int.mone)
-  | eval_static_operation_case28 n1 n2 =>
+  | eval_static_operation_case32 n1 n2 => (* Onxor, I n1 :: I n2 :: nil *) 
       I(Int.xor (Int.xor n1 n2) Int.mone)
-  | eval_static_operation_case29 n1 n2 =>
+  | eval_static_operation_case33 n1 n2 => (* Oshl, I n1 :: I n2 :: nil *) 
       if Int.ltu n2 Int.iwordsize then I(Int.shl n1 n2) else Unknown
-  | eval_static_operation_case30 n1 n2 =>
+  | eval_static_operation_case34 n1 n2 => (* Oshr, I n1 :: I n2 :: nil *) 
       if Int.ltu n2 Int.iwordsize then I(Int.shr n1 n2) else Unknown
-  | eval_static_operation_case31 n n1 =>
+  | eval_static_operation_case35 n n1 => (* Oshrimm n, I n1 :: nil *) 
       if Int.ltu n Int.iwordsize then I(Int.shr n1 n) else Unknown
-  | eval_static_operation_case32 n n1 =>
+  | eval_static_operation_case36 n n1 => (* Oshrximm n, I n1 :: nil *) 
       if Int.ltu n Int.iwordsize then I(Int.shrx n1 n) else Unknown
-  | eval_static_operation_case33 n1 n2 =>
+  | eval_static_operation_case37 n1 n2 => (* Oshru, I n1 :: I n2 :: nil *) 
       if Int.ltu n2 Int.iwordsize then I(Int.shru n1 n2) else Unknown
-  | eval_static_operation_case34 amount mask n1 =>
+  | eval_static_operation_case38 amount mask n1 => (* Orolm amount mask, I n1 :: nil *) 
       I(Int.rolm n1 amount mask)
-  | eval_static_operation_case35 n1 =>
+  | eval_static_operation_case39 amount mask n1 n2 => (* Oroli amount mask, I n1 :: I n2 :: nil *) 
+      I(Int.or (Int.and n1 (Int.not mask)) (Int.rolm n2 amount mask))
+  | eval_static_operation_case40 n1 => (* Onegf, F n1 :: nil *) 
       F(Float.neg n1)
-  | eval_static_operation_case36 n1 =>
+  | eval_static_operation_case41 n1 => (* Oabsf, F n1 :: nil *) 
       F(Float.abs n1)
-  | eval_static_operation_case37 n1 n2 =>
+  | eval_static_operation_case42 n1 n2 => (* Oaddf, F n1 :: F n2 :: nil *) 
       F(Float.add n1 n2)
-  | eval_static_operation_case38 n1 n2 =>
+  | eval_static_operation_case43 n1 n2 => (* Osubf, F n1 :: F n2 :: nil *) 
       F(Float.sub n1 n2)
-  | eval_static_operation_case39 n1 n2 =>
+  | eval_static_operation_case44 n1 n2 => (* Omulf, F n1 :: F n2 :: nil *) 
       F(Float.mul n1 n2)
-  | eval_static_operation_case40 n1 n2 =>
+  | eval_static_operation_case45 n1 n2 => (* Odivf, F n1 :: F n2 :: nil *) 
       F(Float.div n1 n2)
-  | eval_static_operation_case41 n1 n2 n3 =>
+  | eval_static_operation_case46 n1 n2 n3 => (* Omuladdf, F n1 :: F n2 :: F n3 :: nil *) 
       F(Float.add (Float.mul n1 n2) n3)
-  | eval_static_operation_case42 n1 n2 n3 =>
+  | eval_static_operation_case47 n1 n2 n3 => (* Omulsubf, F n1 :: F n2 :: F n3 :: nil *) 
       F(Float.sub (Float.mul n1 n2) n3)
-  | eval_static_operation_case43 n1 =>
+  | eval_static_operation_case48 n1 => (* Osingleoffloat, F n1 :: nil *) 
       F(Float.singleoffloat n1)
-  | eval_static_operation_case44 n1 =>
-      match Float.intoffloat n1 with Some x => I x | None => Unknown end
-  | eval_static_operation_case45 n1 n2 =>
+  | eval_static_operation_case49 n1 => (* Ointoffloat, F n1 :: nil *) 
+      eval_static_intoffloat n1
+  | eval_static_operation_case50 n1 n2 => (* Ofloatofwords, I n1 :: I n2 :: nil *) 
       F(Float.from_words n1 n2)
-  | eval_static_operation_case47 c vl =>
-      match eval_static_condition c vl with
-      | None => Unknown
-      | Some b => I(if b then Int.one else Int.zero)
-      end
-  | eval_static_operation_case48 n1 =>
-      I(Int.zero_ext 8 n1)
-  | eval_static_operation_case49 n1 =>
-      I(Int.zero_ext 16 n1)
+  | eval_static_operation_case51 c vl => (* Ocmp c, vl *) 
+      eval_static_condition_val c vl
   | eval_static_operation_default op vl =>
       Unknown
   end.
+
 
 (** * Operator strength reduction *)
 
@@ -543,87 +409,104 @@ Definition eval_static_operation (op: operation) (vl: list approx) :=
 
 Section STRENGTH_REDUCTION.
 
-Variable app: reg -> approx.
-
-Definition intval (r: reg) : option int :=
-  match app r with I n => Some n | _ => None end.
-
-Inductive cond_strength_reduction_cases: condition -> list reg -> Type :=
-  | csr_case1:
-      forall c r1 r2,
-      cond_strength_reduction_cases (Ccomp c) (r1 :: r2 :: nil)
-  | csr_case2:
-      forall c r1 r2,
-      cond_strength_reduction_cases (Ccompu c) (r1 :: r2 :: nil)
-  | csr_default:
-      forall c rl,
-      cond_strength_reduction_cases c rl.
-
-Definition cond_strength_reduction_match (cond: condition) (rl: list reg) :=
-  match cond as x, rl as y return cond_strength_reduction_cases x y with
-  | Ccomp c, r1 :: r2 :: nil =>
-      csr_case1 c r1 r2
-  | Ccompu c, r1 :: r2 :: nil =>
-      csr_case2 c r1 r2
-  | cond, rl =>
-      csr_default cond rl
-  end.
-
-Definition cond_strength_reduction
-              (cond: condition) (args: list reg) : condition * list reg :=
-  match cond_strength_reduction_match cond args with
-  | csr_case1 c r1 r2 =>
-      match intval r1, intval r2 with
-      | Some n, _ =>
-          (Ccompimm (swap_comparison c) n, r2 :: nil)
-      | _, Some n =>
-          (Ccompimm c n, r1 :: nil)
-      | _, _ =>
-          (cond, args)
-      end
-  | csr_case2 c r1 r2 =>
-      match intval r1, intval r2 with
-      | Some n, _ =>
-          (Ccompuimm (swap_comparison c) n, r2 :: nil)
-      | _, Some n =>
-          (Ccompuimm c n, r1 :: nil)
-      | _, _ =>
-          (cond, args)
-      end
-  | csr_default cond args =>
+(** Original definition:
+<<
+Nondetfunction cond_strength_reduction 
+              (cond: condition) (args: list reg) (vl: list approx) :=
+  match cond, args, vl with
+  | Ccomp c, r1 :: r2 :: nil, I n1 :: v2 :: nil =>
+      (Ccompimm (swap_comparison c) n1, r2 :: nil)
+  | Ccomp c, r1 :: r2 :: nil, v1 :: I n2 :: nil =>
+      (Ccompimm c n2, r1 :: nil)
+  | Ccompu c, r1 :: r2 :: nil, I n1 :: v2 :: nil =>
+      (Ccompuimm (swap_comparison c) n1, r2 :: nil)
+  | Ccompu c, r1 :: r2 :: nil, v1 :: I n2 :: nil =>
+      (Ccompuimm c n2, r1 :: nil)
+  | _, _, _ => 
       (cond, args)
   end.
+>>
+*)
+
+Inductive cond_strength_reduction_cases: forall (cond: condition) (args: list reg) (vl: list approx), Type :=
+  | cond_strength_reduction_case1: forall c r1 r2 n1 v2, cond_strength_reduction_cases (Ccomp c) (r1 :: r2 :: nil) (I n1 :: v2 :: nil)
+  | cond_strength_reduction_case2: forall c r1 r2 v1 n2, cond_strength_reduction_cases (Ccomp c) (r1 :: r2 :: nil) (v1 :: I n2 :: nil)
+  | cond_strength_reduction_case3: forall c r1 r2 n1 v2, cond_strength_reduction_cases (Ccompu c) (r1 :: r2 :: nil) (I n1 :: v2 :: nil)
+  | cond_strength_reduction_case4: forall c r1 r2 v1 n2, cond_strength_reduction_cases (Ccompu c) (r1 :: r2 :: nil) (v1 :: I n2 :: nil)
+  | cond_strength_reduction_default: forall (cond: condition) (args: list reg) (vl: list approx), cond_strength_reduction_cases cond args vl.
+
+Definition cond_strength_reduction_match (cond: condition) (args: list reg) (vl: list approx) :=
+  match cond as zz1, args as zz2, vl as zz3 return cond_strength_reduction_cases zz1 zz2 zz3 with
+  | Ccomp c, r1 :: r2 :: nil, I n1 :: v2 :: nil => cond_strength_reduction_case1 c r1 r2 n1 v2
+  | Ccomp c, r1 :: r2 :: nil, v1 :: I n2 :: nil => cond_strength_reduction_case2 c r1 r2 v1 n2
+  | Ccompu c, r1 :: r2 :: nil, I n1 :: v2 :: nil => cond_strength_reduction_case3 c r1 r2 n1 v2
+  | Ccompu c, r1 :: r2 :: nil, v1 :: I n2 :: nil => cond_strength_reduction_case4 c r1 r2 v1 n2
+  | cond, args, vl => cond_strength_reduction_default cond args vl
+  end.
+
+Definition cond_strength_reduction (cond: condition) (args: list reg) (vl: list approx) :=
+  match cond_strength_reduction_match cond args vl with
+  | cond_strength_reduction_case1 c r1 r2 n1 v2 => (* Ccomp c, r1 :: r2 :: nil, I n1 :: v2 :: nil *) 
+      (Ccompimm (swap_comparison c) n1, r2 :: nil)
+  | cond_strength_reduction_case2 c r1 r2 v1 n2 => (* Ccomp c, r1 :: r2 :: nil, v1 :: I n2 :: nil *) 
+      (Ccompimm c n2, r1 :: nil)
+  | cond_strength_reduction_case3 c r1 r2 n1 v2 => (* Ccompu c, r1 :: r2 :: nil, I n1 :: v2 :: nil *) 
+      (Ccompuimm (swap_comparison c) n1, r2 :: nil)
+  | cond_strength_reduction_case4 c r1 r2 v1 n2 => (* Ccompu c, r1 :: r2 :: nil, v1 :: I n2 :: nil *) 
+      (Ccompuimm c n2, r1 :: nil)
+  | cond_strength_reduction_default cond args vl =>
+      (cond, args)
+  end.
+
 
 Definition make_addimm (n: int) (r: reg) :=
   if Int.eq n Int.zero
   then (Omove, r :: nil)
   else (Oaddimm n, r :: nil).
 
-Definition make_shlimm (n: int) (r: reg) :=
-  if Int.eq n Int.zero
-  then (Omove, r :: nil)
-  else (Orolm n (Int.shl Int.mone n), r :: nil).
+Definition make_shlimm (n: int) (r1 r2: reg) :=
+  if Int.eq n Int.zero then
+    (Omove, r1 :: nil)
+  else if Int.ltu n Int.iwordsize then
+    (Orolm n (Int.shl Int.mone n), r1 :: nil)
+  else
+    (Oshl, r1 :: r2 :: nil).
 
-Definition make_shrimm (n: int) (r: reg) :=
+Definition make_shrimm (n: int) (r1 r2: reg) :=
   if Int.eq n Int.zero
-  then (Omove, r :: nil)
-  else (Oshrimm n, r :: nil).
+  then (Omove, r1 :: nil)
+  else (Oshrimm n, r1 :: nil).
 
-Definition make_shruimm (n: int) (r: reg) :=
-  if Int.eq n Int.zero
-  then (Omove, r :: nil)
-  else (Orolm (Int.sub Int.iwordsize n) (Int.shru Int.mone n), r :: nil).
+Definition make_shruimm (n: int) (r1 r2: reg) :=
+  if Int.eq n Int.zero then
+    (Omove, r1 :: nil)
+  else if Int.ltu n Int.iwordsize then
+    (Orolm (Int.sub Int.iwordsize n) (Int.shru Int.mone n), r1 :: nil)
+  else
+    (Oshru, r1 :: r2 :: nil).
 
-Definition make_mulimm (n: int) (r: reg) :=
+Definition make_mulimm (n: int) (r1 r2: reg) :=
   if Int.eq n Int.zero then
     (Ointconst Int.zero, nil)
   else if Int.eq n Int.one then
-    (Omove, r :: nil)
+    (Omove, r1 :: nil)
   else
     match Int.is_power2 n with
-    | Some l => make_shlimm l r
-    | None => (Omulimm n, r :: nil)
+    | Some l => (Orolm l (Int.shl Int.mone l), r1 :: nil)
+    | None => (Omulimm n, r1 :: nil)
     end.
+
+Definition make_divimm (n: int) (r1 r2: reg) :=
+  match Int.is_power2 n with
+  | Some l => (Oshrximm l, r1 :: nil)
+  | None   => (Odiv, r1 :: r2 :: nil)
+  end.
+
+Definition make_divuimm (n: int) (r1 r2: reg) :=
+  match Int.is_power2 n with
+  | Some l => (Orolm (Int.sub Int.iwordsize l) (Int.shru Int.mone l), r1 :: nil)
+  | None   => (Odivu, r1 :: r2 :: nil)
+  end.
 
 Definition make_andimm (n: int) (r: reg) :=
   if Int.eq n Int.zero
@@ -641,216 +524,212 @@ Definition make_xorimm (n: int) (r: reg) :=
   then (Omove, r :: nil)
   else (Oxorimm n, r :: nil).
 
-Inductive op_strength_reduction_cases: operation -> list reg -> Type :=
-  | op_strength_reduction_case1:
-      forall (r1: reg) (r2: reg),
-      op_strength_reduction_cases Oadd (r1 :: r2 :: nil)
-  | op_strength_reduction_case2:
-      forall (r1: reg) (r2: reg),
-      op_strength_reduction_cases Osub (r1 :: r2 :: nil)
-  | op_strength_reduction_case3:
-      forall (r1: reg) (r2: reg),
-      op_strength_reduction_cases Omul (r1 :: r2 :: nil)
-  | op_strength_reduction_case4:
-      forall (r1: reg) (r2: reg),
-      op_strength_reduction_cases Odiv (r1 :: r2 :: nil)
-  | op_strength_reduction_case5:
-      forall (r1: reg) (r2: reg),
-      op_strength_reduction_cases Odivu (r1 :: r2 :: nil)
-  | op_strength_reduction_case6:
-      forall (r1: reg) (r2: reg),
-      op_strength_reduction_cases Oand (r1 :: r2 :: nil)
-  | op_strength_reduction_case7:
-      forall (r1: reg) (r2: reg),
-      op_strength_reduction_cases Oor (r1 :: r2 :: nil)
-  | op_strength_reduction_case8:
-      forall (r1: reg) (r2: reg),
-      op_strength_reduction_cases Oxor (r1 :: r2 :: nil)
-  | op_strength_reduction_case9:
-      forall (r1: reg) (r2: reg),
-      op_strength_reduction_cases Oshl (r1 :: r2 :: nil)
-  | op_strength_reduction_case10:
-      forall (r1: reg) (r2: reg),
-      op_strength_reduction_cases Oshr (r1 :: r2 :: nil)
-  | op_strength_reduction_case11:
-      forall (r1: reg) (r2: reg),
-      op_strength_reduction_cases Oshru (r1 :: r2 :: nil)
-  | op_strength_reduction_case12:
-      forall (c: condition) (rl: list reg),
-      op_strength_reduction_cases (Ocmp c) rl
-  | op_strength_reduction_default:
-      forall (op: operation) (args: list reg),
-      op_strength_reduction_cases op args.
+(** Original definition:
+<<
+Nondetfunction op_strength_reduction 
+              (op: operation) (args: list reg) (vl: list approx) :=
+  match op, args, vl with
+  | Oadd, r1 :: r2 :: nil, I n1 :: v2 :: nil => make_addimm n1 r2
+  | Oadd, r1 :: r2 :: nil, v1 :: I n2 :: nil => make_addimm n2 r1
+  | Osub, r1 :: r2 :: nil, I n1 :: v2 :: nil => (Osubimm n1, r2 :: nil)
+  | Osub, r1 :: r2 :: nil, v1 :: I n2 :: nil => make_addimm (Int.neg n2) r1
+  | Omul, r1 :: r2 :: nil, I n1 :: v2 :: nil => make_mulimm n1 r2 r1
+  | Omul, r1 :: r2 :: nil, v1 :: I n2 :: nil => make_mulimm n2 r1 r2
+  | Odiv, r1 :: r2 :: nil, v1 :: I n2 :: nil => make_divimm n2 r1 r2
+  | Odivu, r1 :: r2 :: nil, v1 :: I n2 :: nil => make_divuimm n2 r1 r2
+  | Oand, r1 :: r2 :: nil, I n1 :: v2 :: nil => make_andimm n1 r2
+  | Oand, r1 :: r2 :: nil, v1 :: I n2 :: nil => make_andimm n2 r1
+  | Oor, r1 :: r2 :: nil, I n1 :: v2 :: nil => make_orimm n1 r2
+  | Oor, r1 :: r2 :: nil, v1 :: I n2 :: nil => make_orimm n2 r1
+  | Oxor, r1 :: r2 :: nil, I n1 :: v2 :: nil => make_xorimm n1 r2
+  | Oxor, r1 :: r2 :: nil, v1 :: I n2 :: nil => make_xorimm n2 r1
+  | Oshl, r1 :: r2 :: nil, v1 :: I n2 :: nil => make_shlimm n2 r1 r2
+  | Oshr, r1 :: r2 :: nil, v1 :: I n2 :: nil => make_shrimm n2 r1 r2
+  | Oshru, r1 :: r2 :: nil, v1 :: I n2 :: nil => make_shruimm n2 r1 r2
+  | Ocmp c, args, vl =>
+      let (c', args') := cond_strength_reduction c args vl in (Ocmp c', args')
+  | _, _, _ => (op, args)
+  end.
+>>
+*)
 
-Definition op_strength_reduction_match (op: operation) (args: list reg) :=
-  match op as z1, args as z2 return op_strength_reduction_cases z1 z2 with
-  | Oadd, r1 :: r2 :: nil =>
-      op_strength_reduction_case1 r1 r2
-  | Osub, r1 :: r2 :: nil =>
-      op_strength_reduction_case2 r1 r2
-  | Omul, r1 :: r2 :: nil =>
-      op_strength_reduction_case3 r1 r2
-  | Odiv, r1 :: r2 :: nil =>
-      op_strength_reduction_case4 r1 r2
-  | Odivu, r1 :: r2 :: nil =>
-      op_strength_reduction_case5 r1 r2
-  | Oand, r1 :: r2 :: nil =>
-      op_strength_reduction_case6 r1 r2
-  | Oor, r1 :: r2 :: nil =>
-      op_strength_reduction_case7 r1 r2
-  | Oxor, r1 :: r2 :: nil =>
-      op_strength_reduction_case8 r1 r2
-  | Oshl, r1 :: r2 :: nil =>
-      op_strength_reduction_case9 r1 r2
-  | Oshr, r1 :: r2 :: nil =>
-      op_strength_reduction_case10 r1 r2
-  | Oshru, r1 :: r2 :: nil =>
-      op_strength_reduction_case11 r1 r2
-  | Ocmp c, rl =>
-      op_strength_reduction_case12 c rl
-  | op, args =>
-      op_strength_reduction_default op args
+Inductive op_strength_reduction_cases: forall (op: operation) (args: list reg) (vl: list approx), Type :=
+  | op_strength_reduction_case1: forall r1 r2 n1 v2, op_strength_reduction_cases (Oadd) (r1 :: r2 :: nil) (I n1 :: v2 :: nil)
+  | op_strength_reduction_case2: forall r1 r2 v1 n2, op_strength_reduction_cases (Oadd) (r1 :: r2 :: nil) (v1 :: I n2 :: nil)
+  | op_strength_reduction_case3: forall r1 r2 n1 v2, op_strength_reduction_cases (Osub) (r1 :: r2 :: nil) (I n1 :: v2 :: nil)
+  | op_strength_reduction_case4: forall r1 r2 v1 n2, op_strength_reduction_cases (Osub) (r1 :: r2 :: nil) (v1 :: I n2 :: nil)
+  | op_strength_reduction_case5: forall r1 r2 n1 v2, op_strength_reduction_cases (Omul) (r1 :: r2 :: nil) (I n1 :: v2 :: nil)
+  | op_strength_reduction_case6: forall r1 r2 v1 n2, op_strength_reduction_cases (Omul) (r1 :: r2 :: nil) (v1 :: I n2 :: nil)
+  | op_strength_reduction_case7: forall r1 r2 v1 n2, op_strength_reduction_cases (Odiv) (r1 :: r2 :: nil) (v1 :: I n2 :: nil)
+  | op_strength_reduction_case8: forall r1 r2 v1 n2, op_strength_reduction_cases (Odivu) (r1 :: r2 :: nil) (v1 :: I n2 :: nil)
+  | op_strength_reduction_case9: forall r1 r2 n1 v2, op_strength_reduction_cases (Oand) (r1 :: r2 :: nil) (I n1 :: v2 :: nil)
+  | op_strength_reduction_case10: forall r1 r2 v1 n2, op_strength_reduction_cases (Oand) (r1 :: r2 :: nil) (v1 :: I n2 :: nil)
+  | op_strength_reduction_case11: forall r1 r2 n1 v2, op_strength_reduction_cases (Oor) (r1 :: r2 :: nil) (I n1 :: v2 :: nil)
+  | op_strength_reduction_case12: forall r1 r2 v1 n2, op_strength_reduction_cases (Oor) (r1 :: r2 :: nil) (v1 :: I n2 :: nil)
+  | op_strength_reduction_case13: forall r1 r2 n1 v2, op_strength_reduction_cases (Oxor) (r1 :: r2 :: nil) (I n1 :: v2 :: nil)
+  | op_strength_reduction_case14: forall r1 r2 v1 n2, op_strength_reduction_cases (Oxor) (r1 :: r2 :: nil) (v1 :: I n2 :: nil)
+  | op_strength_reduction_case15: forall r1 r2 v1 n2, op_strength_reduction_cases (Oshl) (r1 :: r2 :: nil) (v1 :: I n2 :: nil)
+  | op_strength_reduction_case16: forall r1 r2 v1 n2, op_strength_reduction_cases (Oshr) (r1 :: r2 :: nil) (v1 :: I n2 :: nil)
+  | op_strength_reduction_case17: forall r1 r2 v1 n2, op_strength_reduction_cases (Oshru) (r1 :: r2 :: nil) (v1 :: I n2 :: nil)
+  | op_strength_reduction_case18: forall c args vl, op_strength_reduction_cases (Ocmp c) (args) (vl)
+  | op_strength_reduction_default: forall (op: operation) (args: list reg) (vl: list approx), op_strength_reduction_cases op args vl.
+
+Definition op_strength_reduction_match (op: operation) (args: list reg) (vl: list approx) :=
+  match op as zz1, args as zz2, vl as zz3 return op_strength_reduction_cases zz1 zz2 zz3 with
+  | Oadd, r1 :: r2 :: nil, I n1 :: v2 :: nil => op_strength_reduction_case1 r1 r2 n1 v2
+  | Oadd, r1 :: r2 :: nil, v1 :: I n2 :: nil => op_strength_reduction_case2 r1 r2 v1 n2
+  | Osub, r1 :: r2 :: nil, I n1 :: v2 :: nil => op_strength_reduction_case3 r1 r2 n1 v2
+  | Osub, r1 :: r2 :: nil, v1 :: I n2 :: nil => op_strength_reduction_case4 r1 r2 v1 n2
+  | Omul, r1 :: r2 :: nil, I n1 :: v2 :: nil => op_strength_reduction_case5 r1 r2 n1 v2
+  | Omul, r1 :: r2 :: nil, v1 :: I n2 :: nil => op_strength_reduction_case6 r1 r2 v1 n2
+  | Odiv, r1 :: r2 :: nil, v1 :: I n2 :: nil => op_strength_reduction_case7 r1 r2 v1 n2
+  | Odivu, r1 :: r2 :: nil, v1 :: I n2 :: nil => op_strength_reduction_case8 r1 r2 v1 n2
+  | Oand, r1 :: r2 :: nil, I n1 :: v2 :: nil => op_strength_reduction_case9 r1 r2 n1 v2
+  | Oand, r1 :: r2 :: nil, v1 :: I n2 :: nil => op_strength_reduction_case10 r1 r2 v1 n2
+  | Oor, r1 :: r2 :: nil, I n1 :: v2 :: nil => op_strength_reduction_case11 r1 r2 n1 v2
+  | Oor, r1 :: r2 :: nil, v1 :: I n2 :: nil => op_strength_reduction_case12 r1 r2 v1 n2
+  | Oxor, r1 :: r2 :: nil, I n1 :: v2 :: nil => op_strength_reduction_case13 r1 r2 n1 v2
+  | Oxor, r1 :: r2 :: nil, v1 :: I n2 :: nil => op_strength_reduction_case14 r1 r2 v1 n2
+  | Oshl, r1 :: r2 :: nil, v1 :: I n2 :: nil => op_strength_reduction_case15 r1 r2 v1 n2
+  | Oshr, r1 :: r2 :: nil, v1 :: I n2 :: nil => op_strength_reduction_case16 r1 r2 v1 n2
+  | Oshru, r1 :: r2 :: nil, v1 :: I n2 :: nil => op_strength_reduction_case17 r1 r2 v1 n2
+  | Ocmp c, args, vl => op_strength_reduction_case18 c args vl
+  | op, args, vl => op_strength_reduction_default op args vl
   end.
 
-Definition op_strength_reduction (op: operation) (args: list reg) :=
-  match op_strength_reduction_match op args with
-  | op_strength_reduction_case1 r1 r2 => (* Oadd *)
-      match intval r1, intval r2 with
-      | Some n, _ => make_addimm n r2
-      | _, Some n => make_addimm n r1
-      | _, _ => (op, args)
-      end
-  | op_strength_reduction_case2 r1 r2 => (* Osub *)
-      match intval r1, intval r2 with
-      | Some n, _ => (Osubimm n, r2 :: nil)
-      | _, Some n => make_addimm (Int.neg n) r1
-      | _, _ => (op, args)
-      end
-  | op_strength_reduction_case3 r1 r2 => (* Omul *)
-      match intval r1, intval r2 with
-      | Some n, _ => make_mulimm n r2
-      | _, Some n => make_mulimm n r1
-      | _, _ => (op, args)
-      end
-  | op_strength_reduction_case4 r1 r2 => (* Odiv *)
-      match intval r2 with
-      | Some n =>
-          match Int.is_power2 n with
-          | Some l => (Oshrximm l, r1 :: nil)
-          | None   => (op, args)
-          end
-      | None =>
-          (op, args)
-      end
-  | op_strength_reduction_case5 r1 r2 => (* Odivu *)
-      match intval r2 with
-      | Some n =>
-          match Int.is_power2 n with
-          | Some l => make_shruimm l r1
-          | None   => (op, args)
-          end
-      | None =>
-          (op, args)
-      end
-  | op_strength_reduction_case6 r1 r2 => (* Oand *)
-      match intval r1, intval r2 with
-      | Some n, _ => make_andimm n r2
-      | _, Some n => make_andimm n r1
-      | _, _ => (op, args)
-      end
-  | op_strength_reduction_case7 r1 r2 => (* Oor *)
-      match intval r1, intval r2 with
-      | Some n, _ => make_orimm n r2
-      | _, Some n => make_orimm n r1
-      | _, _ => (op, args)
-      end
-  | op_strength_reduction_case8 r1 r2 => (* Oxor *)
-      match intval r1, intval r2 with
-      | Some n, _ => make_xorimm n r2
-      | _, Some n => make_xorimm n r1
-      | _, _ => (op, args)
-      end
-  | op_strength_reduction_case9 r1 r2 => (* Oshl *)
-      match intval r2 with
-      | Some n =>
-          if Int.ltu n Int.iwordsize
-          then make_shlimm n r1
-          else (op, args)
-      | _ => (op, args)
-      end
-  | op_strength_reduction_case10 r1 r2 => (* Oshr *)
-      match intval r2 with
-      | Some n =>
-          if Int.ltu n Int.iwordsize
-          then make_shrimm n r1
-          else (op, args)
-      | _ => (op, args)
-      end
-  | op_strength_reduction_case11 r1 r2 => (* Oshru *)
-      match intval r2 with
-      | Some n =>
-          if Int.ltu n Int.iwordsize
-          then make_shruimm n r1
-          else (op, args)
-      | _ => (op, args)
-      end
-  | op_strength_reduction_case12 c args => (* Ocmp *)
-      let (c', args') := cond_strength_reduction c args in
-      (Ocmp c', args')
-  | op_strength_reduction_default op args => (* default *)
+Definition op_strength_reduction (op: operation) (args: list reg) (vl: list approx) :=
+  match op_strength_reduction_match op args vl with
+  | op_strength_reduction_case1 r1 r2 n1 v2 => (* Oadd, r1 :: r2 :: nil, I n1 :: v2 :: nil *) 
+      make_addimm n1 r2
+  | op_strength_reduction_case2 r1 r2 v1 n2 => (* Oadd, r1 :: r2 :: nil, v1 :: I n2 :: nil *) 
+      make_addimm n2 r1
+  | op_strength_reduction_case3 r1 r2 n1 v2 => (* Osub, r1 :: r2 :: nil, I n1 :: v2 :: nil *) 
+      (Osubimm n1, r2 :: nil)
+  | op_strength_reduction_case4 r1 r2 v1 n2 => (* Osub, r1 :: r2 :: nil, v1 :: I n2 :: nil *) 
+      make_addimm (Int.neg n2) r1
+  | op_strength_reduction_case5 r1 r2 n1 v2 => (* Omul, r1 :: r2 :: nil, I n1 :: v2 :: nil *) 
+      make_mulimm n1 r2 r1
+  | op_strength_reduction_case6 r1 r2 v1 n2 => (* Omul, r1 :: r2 :: nil, v1 :: I n2 :: nil *) 
+      make_mulimm n2 r1 r2
+  | op_strength_reduction_case7 r1 r2 v1 n2 => (* Odiv, r1 :: r2 :: nil, v1 :: I n2 :: nil *) 
+      make_divimm n2 r1 r2
+  | op_strength_reduction_case8 r1 r2 v1 n2 => (* Odivu, r1 :: r2 :: nil, v1 :: I n2 :: nil *) 
+      make_divuimm n2 r1 r2
+  | op_strength_reduction_case9 r1 r2 n1 v2 => (* Oand, r1 :: r2 :: nil, I n1 :: v2 :: nil *) 
+      make_andimm n1 r2
+  | op_strength_reduction_case10 r1 r2 v1 n2 => (* Oand, r1 :: r2 :: nil, v1 :: I n2 :: nil *) 
+      make_andimm n2 r1
+  | op_strength_reduction_case11 r1 r2 n1 v2 => (* Oor, r1 :: r2 :: nil, I n1 :: v2 :: nil *) 
+      make_orimm n1 r2
+  | op_strength_reduction_case12 r1 r2 v1 n2 => (* Oor, r1 :: r2 :: nil, v1 :: I n2 :: nil *) 
+      make_orimm n2 r1
+  | op_strength_reduction_case13 r1 r2 n1 v2 => (* Oxor, r1 :: r2 :: nil, I n1 :: v2 :: nil *) 
+      make_xorimm n1 r2
+  | op_strength_reduction_case14 r1 r2 v1 n2 => (* Oxor, r1 :: r2 :: nil, v1 :: I n2 :: nil *) 
+      make_xorimm n2 r1
+  | op_strength_reduction_case15 r1 r2 v1 n2 => (* Oshl, r1 :: r2 :: nil, v1 :: I n2 :: nil *) 
+      make_shlimm n2 r1 r2
+  | op_strength_reduction_case16 r1 r2 v1 n2 => (* Oshr, r1 :: r2 :: nil, v1 :: I n2 :: nil *) 
+      make_shrimm n2 r1 r2
+  | op_strength_reduction_case17 r1 r2 v1 n2 => (* Oshru, r1 :: r2 :: nil, v1 :: I n2 :: nil *) 
+      make_shruimm n2 r1 r2
+  | op_strength_reduction_case18 c args vl => (* Ocmp c, args, vl *) 
+      let (c', args') := cond_strength_reduction c args vl in (Ocmp c', args')
+  | op_strength_reduction_default op args vl =>
       (op, args)
   end.
 
-Inductive addr_strength_reduction_cases: forall (addr: addressing) (args: list reg), Type :=
-  | addr_strength_reduction_case1:
-      forall (r1: reg) (r2: reg),
-      addr_strength_reduction_cases (Aindexed2) (r1 :: r2 :: nil)
-  | addr_strength_reduction_case2:
-      forall (symb: ident) (ofs: int) (r1: reg),
-      addr_strength_reduction_cases (Abased symb ofs) (r1 :: nil)
-  | addr_strength_reduction_case3:
-      forall n r1,
-      addr_strength_reduction_cases (Aindexed n) (r1 :: nil)
-  | addr_strength_reduction_default:
-      forall (addr: addressing) (args: list reg),
-      addr_strength_reduction_cases addr args.
 
-Definition addr_strength_reduction_match (addr: addressing) (args: list reg) :=
-  match addr as z1, args as z2 return addr_strength_reduction_cases z1 z2 with
-  | Aindexed2, r1 :: r2 :: nil =>
-      addr_strength_reduction_case1 r1 r2
-  | Abased symb ofs, r1 :: nil =>
-      addr_strength_reduction_case2 symb ofs r1
-  | Aindexed n, r1 :: nil =>
-      addr_strength_reduction_case3 n r1
-  | addr, args =>
-      addr_strength_reduction_default addr args
-  end.
-
-Definition addr_strength_reduction (addr: addressing) (args: list reg) :=
-  match addr_strength_reduction_match addr args with
-  | addr_strength_reduction_case1 r1 r2 => (* Aindexed2 *)
-      match app r1, app r2 with
-      | S symb n1, I n2 => (Aglobal symb (Int.add n1 n2), nil)
-      | S symb n1, _ => (Abased symb n1, r2 :: nil)
-      | I n1, S symb n2 => (Aglobal symb (Int.add n1 n2), nil)
-      | I n1, _ => (Aindexed n1, r2 :: nil)
-      | _, S symb n2 => (Abased symb n2, r1 :: nil)
-      | _, I n2 => (Aindexed n2, r1 :: nil)
-      | _, _ => (addr, args)
-      end
-  | addr_strength_reduction_case2 symb ofs r1 => (* Abased *)
-      match intval r1 with
-      | Some n => (Aglobal symb (Int.add ofs n), nil)
-      | _ => (addr, args)
-      end
-  | addr_strength_reduction_case3 n r1 => (* Aindexed *)
-      match app r1 with
-      | S symb ofs => (Aglobal symb (Int.add ofs n), nil)
-      | _ => (addr, args)
-      end
-  | addr_strength_reduction_default addr args => (* default *)
+(** Original definition:
+<<
+Nondetfunction addr_strength_reduction
+                (addr: addressing) (args: list reg) (vl: list approx) :=
+  match addr, args, vl with
+  | Aindexed2, r1 :: r2 :: nil, G symb n1 :: I n2 :: nil =>
+      (Aglobal symb (Int.add n1 n2), nil)
+  | Aindexed2, r1 :: r2 :: nil, I n1 :: G symb n2 :: nil =>
+      (Aglobal symb (Int.add n1 n2), nil)
+  | Aindexed2, r1 :: r2 :: nil, S n1 :: I n2 :: nil =>
+      (Ainstack (Int.add n1 n2), nil)
+  | Aindexed2, r1 :: r2 :: nil, I n1 :: S n2 :: nil =>
+      (Ainstack (Int.add n1 n2), nil)
+  | Aindexed2, r1 :: r2 :: nil, G symb n1 :: v2 :: nil =>
+      (Abased symb n1, r2 :: nil)
+  | Aindexed2, r1 :: r2 :: nil, v1 :: G symb n2 :: nil =>
+      (Abased symb n2, r1 :: nil)
+  | Aindexed2, r1 :: r2 :: nil, I n1 :: v2 :: nil =>
+      (Aindexed n1, r2 :: nil)
+  | Aindexed2, r1 :: r2 :: nil, v1 :: I n2 :: nil =>
+      (Aindexed n2, r1 :: nil)
+  | Abased symb ofs, r1 :: nil, I n1 :: nil =>
+      (Aglobal symb (Int.add ofs n1), nil)
+  | Aindexed n, r1 :: nil, G symb n1 :: nil =>
+      (Aglobal symb (Int.add n1 n), nil)
+  | Aindexed n, r1 :: nil, S n1 :: nil =>
+      (Ainstack (Int.add n1 n), nil)
+  | _, _, _ =>
       (addr, args)
   end.
+>>
+*)
+
+Inductive addr_strength_reduction_cases: forall (addr: addressing) (args: list reg) (vl: list approx), Type :=
+  | addr_strength_reduction_case1: forall r1 r2 symb n1 n2, addr_strength_reduction_cases (Aindexed2) (r1 :: r2 :: nil) (G symb n1 :: I n2 :: nil)
+  | addr_strength_reduction_case2: forall r1 r2 n1 symb n2, addr_strength_reduction_cases (Aindexed2) (r1 :: r2 :: nil) (I n1 :: G symb n2 :: nil)
+  | addr_strength_reduction_case3: forall r1 r2 n1 n2, addr_strength_reduction_cases (Aindexed2) (r1 :: r2 :: nil) (S n1 :: I n2 :: nil)
+  | addr_strength_reduction_case4: forall r1 r2 n1 n2, addr_strength_reduction_cases (Aindexed2) (r1 :: r2 :: nil) (I n1 :: S n2 :: nil)
+  | addr_strength_reduction_case5: forall r1 r2 symb n1 v2, addr_strength_reduction_cases (Aindexed2) (r1 :: r2 :: nil) (G symb n1 :: v2 :: nil)
+  | addr_strength_reduction_case6: forall r1 r2 v1 symb n2, addr_strength_reduction_cases (Aindexed2) (r1 :: r2 :: nil) (v1 :: G symb n2 :: nil)
+  | addr_strength_reduction_case7: forall r1 r2 n1 v2, addr_strength_reduction_cases (Aindexed2) (r1 :: r2 :: nil) (I n1 :: v2 :: nil)
+  | addr_strength_reduction_case8: forall r1 r2 v1 n2, addr_strength_reduction_cases (Aindexed2) (r1 :: r2 :: nil) (v1 :: I n2 :: nil)
+  | addr_strength_reduction_case9: forall symb ofs r1 n1, addr_strength_reduction_cases (Abased symb ofs) (r1 :: nil) (I n1 :: nil)
+  | addr_strength_reduction_case10: forall n r1 symb n1, addr_strength_reduction_cases (Aindexed n) (r1 :: nil) (G symb n1 :: nil)
+  | addr_strength_reduction_case11: forall n r1 n1, addr_strength_reduction_cases (Aindexed n) (r1 :: nil) (S n1 :: nil)
+  | addr_strength_reduction_default: forall (addr: addressing) (args: list reg) (vl: list approx), addr_strength_reduction_cases addr args vl.
+
+Definition addr_strength_reduction_match (addr: addressing) (args: list reg) (vl: list approx) :=
+  match addr as zz1, args as zz2, vl as zz3 return addr_strength_reduction_cases zz1 zz2 zz3 with
+  | Aindexed2, r1 :: r2 :: nil, G symb n1 :: I n2 :: nil => addr_strength_reduction_case1 r1 r2 symb n1 n2
+  | Aindexed2, r1 :: r2 :: nil, I n1 :: G symb n2 :: nil => addr_strength_reduction_case2 r1 r2 n1 symb n2
+  | Aindexed2, r1 :: r2 :: nil, S n1 :: I n2 :: nil => addr_strength_reduction_case3 r1 r2 n1 n2
+  | Aindexed2, r1 :: r2 :: nil, I n1 :: S n2 :: nil => addr_strength_reduction_case4 r1 r2 n1 n2
+  | Aindexed2, r1 :: r2 :: nil, G symb n1 :: v2 :: nil => addr_strength_reduction_case5 r1 r2 symb n1 v2
+  | Aindexed2, r1 :: r2 :: nil, v1 :: G symb n2 :: nil => addr_strength_reduction_case6 r1 r2 v1 symb n2
+  | Aindexed2, r1 :: r2 :: nil, I n1 :: v2 :: nil => addr_strength_reduction_case7 r1 r2 n1 v2
+  | Aindexed2, r1 :: r2 :: nil, v1 :: I n2 :: nil => addr_strength_reduction_case8 r1 r2 v1 n2
+  | Abased symb ofs, r1 :: nil, I n1 :: nil => addr_strength_reduction_case9 symb ofs r1 n1
+  | Aindexed n, r1 :: nil, G symb n1 :: nil => addr_strength_reduction_case10 n r1 symb n1
+  | Aindexed n, r1 :: nil, S n1 :: nil => addr_strength_reduction_case11 n r1 n1
+  | addr, args, vl => addr_strength_reduction_default addr args vl
+  end.
+
+Definition addr_strength_reduction (addr: addressing) (args: list reg) (vl: list approx) :=
+  match addr_strength_reduction_match addr args vl with
+  | addr_strength_reduction_case1 r1 r2 symb n1 n2 => (* Aindexed2, r1 :: r2 :: nil, G symb n1 :: I n2 :: nil *) 
+      (Aglobal symb (Int.add n1 n2), nil)
+  | addr_strength_reduction_case2 r1 r2 n1 symb n2 => (* Aindexed2, r1 :: r2 :: nil, I n1 :: G symb n2 :: nil *) 
+      (Aglobal symb (Int.add n1 n2), nil)
+  | addr_strength_reduction_case3 r1 r2 n1 n2 => (* Aindexed2, r1 :: r2 :: nil, S n1 :: I n2 :: nil *) 
+      (Ainstack (Int.add n1 n2), nil)
+  | addr_strength_reduction_case4 r1 r2 n1 n2 => (* Aindexed2, r1 :: r2 :: nil, I n1 :: S n2 :: nil *) 
+      (Ainstack (Int.add n1 n2), nil)
+  | addr_strength_reduction_case5 r1 r2 symb n1 v2 => (* Aindexed2, r1 :: r2 :: nil, G symb n1 :: v2 :: nil *) 
+      (Abased symb n1, r2 :: nil)
+  | addr_strength_reduction_case6 r1 r2 v1 symb n2 => (* Aindexed2, r1 :: r2 :: nil, v1 :: G symb n2 :: nil *) 
+      (Abased symb n2, r1 :: nil)
+  | addr_strength_reduction_case7 r1 r2 n1 v2 => (* Aindexed2, r1 :: r2 :: nil, I n1 :: v2 :: nil *) 
+      (Aindexed n1, r2 :: nil)
+  | addr_strength_reduction_case8 r1 r2 v1 n2 => (* Aindexed2, r1 :: r2 :: nil, v1 :: I n2 :: nil *) 
+      (Aindexed n2, r1 :: nil)
+  | addr_strength_reduction_case9 symb ofs r1 n1 => (* Abased symb ofs, r1 :: nil, I n1 :: nil *) 
+      (Aglobal symb (Int.add ofs n1), nil)
+  | addr_strength_reduction_case10 n r1 symb n1 => (* Aindexed n, r1 :: nil, G symb n1 :: nil *) 
+      (Aglobal symb (Int.add n1 n), nil)
+  | addr_strength_reduction_case11 n r1 n1 => (* Aindexed n, r1 :: nil, S n1 :: nil *) 
+      (Ainstack (Int.add n1 n), nil)
+  | addr_strength_reduction_default addr args vl =>
+      (addr, args)
+  end.
+
 
 End STRENGTH_REDUCTION.
