powerpc/SelectOpproof.v
@@ -115,21 +115,21 @@ Definition binary_constructor_sound (cstr: expr -> expr -> expr) (sem: val -> va
   exists v, eval_expr ge sp e m le (cstr a b) v /\ Val.lessdef (sem x y) v.
 
 Theorem eval_addrsymbol:
-  forall le id ofs b,
-  Genv.find_symbol ge id = Some b ->
-  eval_expr ge sp e m le (addrsymbol id ofs) (Vptr b ofs).
+  forall le id ofs,
+  exists v, eval_expr ge sp e m le (addrsymbol id ofs) v /\ Val.lessdef (symbol_address ge id ofs) v.
 Proof.
-  intros. unfold addrsymbol. econstructor. constructor. 
-  simpl. unfold symbol_address. rewrite H. auto.
+  intros. unfold addrsymbol. econstructor; split. 
+  EvalOp. simpl; eauto. 
+  auto.
 Qed.
 
 Theorem eval_addrstack:
-  forall le ofs b n,
-  sp = Vptr b n ->
-  eval_expr ge sp e m le (addrstack ofs) (Vptr b (Int.add n ofs)).
+  forall le ofs,
+  exists v, eval_expr ge sp e m le (addrstack ofs) v /\ Val.lessdef (Val.add sp (Vint ofs)) v.
 Proof.
-  intros. unfold addrstack. econstructor. constructor.
-  subst; simpl. auto.
+  intros. unfold addrstack. econstructor; split.
+  EvalOp. simpl; eauto. 
+  auto.
 Qed.
 
 Theorem eval_notint: unary_constructor_sound notint Val.notint.
@@ -148,26 +148,6 @@ Proof.
   simpl. destruct x; simpl; auto. rewrite Int.or_idem. auto.
 Qed.
 
-(*
-Lemma eval_notbool_base: unary_constructor_sound notbool_base Val.notbool.
-
-  forall le a v b,
-  eval_expr ge sp e m le a v ->
-  Val.bool_of_val v b ->
-  eval_expr ge sp e m le (notbool_base a) (Val.of_bool (negb b)).
-Proof. 
-  TrivialOp notbool_base. simpl. 
-  inv H0. 
-  rewrite Int.eq_false; auto.
-  rewrite Int.eq_true; auto.
-  reflexivity.
-Qed.
-*)
-(*
-Hint Resolve Val.bool_of_true_val Val.bool_of_false_val
-             Val.bool_of_true_val_inv Val.bool_of_false_val_inv: valboolof.
-*)
-
 Theorem eval_notbool: unary_constructor_sound notbool Val.notbool.
 Proof.
   assert (DFL: 
@@ -175,7 +155,7 @@ Proof.
     eval_expr ge sp e m le a x ->
      exists v, eval_expr ge sp e m le (Eop (Ocmp (Ccompuimm Ceq Int.zero)) (a ::: Enil)) v
            /\ Val.lessdef (Val.notbool x) v).
-  intros. TrivialExists. simpl. destruct x; simpl; auto. destruct (Int.eq i Int.zero); auto.
+  intros. TrivialExists. simpl. destruct x; simpl; auto.
 
   red. induction a; simpl; intros; eauto. destruct o; eauto.
 (* intconst *)
@@ -249,6 +229,11 @@ Proof.
   TrivialExists.
 Qed.
 
+Theorem eval_negint: unary_constructor_sound negint (fun v => Val.sub Vzero v).
+Proof.
+  red; intros. unfold negint. TrivialExists.
+Qed.
+
 Lemma eval_rolm:
   forall amount mask,
   unary_constructor_sound (fun a => rolm a amount mask)
@@ -296,18 +281,6 @@ Proof.
   TrivialExists. econstructor. eauto. econstructor. EvalOp. simpl; eauto. constructor. auto.
 Qed.
 
-(* Move to Values *)
-
-Lemma val_add_lessdef:
-  forall v1 v1' v2 v2', Val.lessdef v1 v1' -> Val.lessdef v2 v2' -> Val.lessdef (Val.add v1 v2) (Val.add v1' v2').
-Admitted.
-
-Lemma val_lessdef_trans:
-  forall v1 v2 v3, Val.lessdef v1 v2 -> Val.lessdef v2 v3 -> Val.lessdef v1 v3.
-Proof.
-  intros. inv H; auto.
-Qed.
-
 Lemma eval_mulimm_base:
   forall n, unary_constructor_sound (mulimm_base n) (fun x => Val.mul x (Vint n)).
 Proof.
@@ -331,7 +304,7 @@ Proof.
   replace (Vint (Int.add (Int.shl Int.one i) (Int.shl Int.one i0)))
      with (Val.add (Val.shl Vone (Vint i)) (Val.shl Vone (Vint i0))).
   rewrite Val.mul_add_distr_r.
-  repeat rewrite Val.shl_mul. apply val_add_lessdef; auto. 
+  repeat rewrite Val.shl_mul. apply Val.add_lessdef; auto. 
   simpl. repeat rewrite H0; auto with coqlib. 
   intros. TrivialExists. 
 Qed.
@@ -351,7 +324,7 @@ Proof.
   subst. rewrite Val.mul_add_distr_l. 
   exploit eval_mulimm_base; eauto. instantiate (1 := n). intros [v' [A1 B1]].
   exploit (eval_addimm (Int.mul n n2) le (mulimm_base n t2) v'). auto. intros [v'' [A2 B2]].
-  exists v''; split; auto. eapply val_lessdef_trans. eapply val_add_lessdef; eauto. 
+  exists v''; split; auto. eapply Val.lessdef_trans. eapply Val.add_lessdef; eauto. 
   rewrite Val.mul_commut; auto.
   apply eval_mulimm_base; auto.
 Qed.
@@ -374,6 +347,18 @@ Proof.
   InvEval. subst. TrivialExists. simpl. 
   destruct v1; auto. simpl. unfold Int.rolm. rewrite Int.and_assoc. 
   decEq. decEq. decEq. apply Int.and_commut.
+  destruct (Int.eq (Int.shru (Int.shl n amount) amount) n &&
+            Int.ltu amount Int.iwordsize) as []_eqn.
+  InvEval. destruct (andb_prop _ _ Heqb). 
+  generalize (Int.eq_spec (Int.shru (Int.shl n amount) amount) n). rewrite H0; intros.
+  replace (Val.and x (Vint n))
+     with (Val.rolm v1 (Int.sub Int.iwordsize amount) (Int.and (Int.shru Int.mone amount) n)).
+  apply eval_rolm; auto.
+  subst x. destruct v1; simpl; auto. rewrite H1; simpl. decEq. 
+  transitivity (Int.and (Int.shru i amount) n).
+  rewrite (Int.shru_rolm i); auto. unfold Int.rolm. rewrite Int.and_assoc; auto. 
+  symmetry. apply Int.shr_and_shru_and. auto.
+  TrivialExists. 
   TrivialExists.
 Qed.
 
@@ -421,11 +406,15 @@ Proof.
   rewrite Val.or_rolm. TrivialExists.
   TrivialExists.
 (* andimm - rolm *)
-  predSpec Int.eq Int.eq_spec mask1 (Int.not mask2). 
+  destruct (Int.eq mask1 (Int.not mask2) && is_rlw_mask mask2) as []_eqn.
+  destruct (andb_prop _ _ Heqb0). 
+  generalize (Int.eq_spec mask1 (Int.not mask2)); rewrite H1; intros.
   InvEval. subst. TrivialExists. 
   TrivialExists.
 (* rolm - andimm *)
-  predSpec Int.eq Int.eq_spec mask2 (Int.not mask1). 
+  destruct (Int.eq mask2 (Int.not mask1) && is_rlw_mask mask1) as []_eqn.
+  destruct (andb_prop _ _ Heqb0). 
+  generalize (Int.eq_spec mask2 (Int.not mask1)); rewrite H1; intros.
   InvEval. subst. rewrite Val.or_commut. TrivialExists.
   TrivialExists.
 (* intconst *)
@@ -489,15 +478,6 @@ Proof.
   reflexivity.
 Qed.
 
-Theorem val_mods_divs:
-  forall x y z, Val.mods x y = Some z -> exists v, Val.divs x y = Some v /\ z = Val.sub x (Val.mul v y).
-Proof.
-  intros. destruct x; destruct y; simpl in *; try discriminate.
-  destruct (Int.eq i0 Int.zero); inv H. 
-  exists (Vint (Int.divs i i0)); split; auto. 
-  simpl. rewrite Int.mods_divs. auto.
-Qed.
-
 Theorem eval_mods:
   forall le a b x y z,
   eval_expr ge sp e m le a x ->
@@ -506,22 +486,10 @@ Theorem eval_mods:
   exists v, eval_expr ge sp e m le (mods a b) v /\ Val.lessdef z v.
 Proof.
   intros; unfold mods. 
-  exploit val_mods_divs; eauto. intros [v [A B]].
+  exploit Val.mods_divs; eauto. intros [v [A B]].
   subst. econstructor; split; eauto.
   apply eval_mod_aux with (semdivop := Val.divs); auto.
 Qed.
-
-(*
-Lemma eval_divu_base:
-  forall le a b x y z,
-  eval_expr ge sp e m le a x ->
-  eval_expr ge sp e m le b y ->
-  Val.divu x y = Some z ->
-  exists v, eval_expr ge sp e m le (Eop Odivu (a:::b:::Enil)) v /\ Val.lessdef z v.
-Proof.
-  intros. unfold divu. exists z; split. EvalOp. auto.
-Qed.
-*)
 
 Theorem eval_divuimm:
   forall le n a x z,
@@ -549,16 +517,6 @@ Proof.
   TrivialExists. 
 Qed.
 
-Theorem val_modu_divu:
-  forall x y z, Val.modu x y = Some z -> exists v, Val.divu x y = Some v /\ z = Val.sub x (Val.mul v y).
-Proof.
-  intros. destruct x; destruct y; simpl in *; try discriminate.
-  destruct (Int.eq i0 Int.zero) as []_eqn; inv H. 
-  exists (Vint (Int.divu i i0)); split; auto. 
-  simpl. rewrite Int.modu_divu. auto.
-  generalize (Int.eq_spec i0 Int.zero). rewrite Heqb; auto. 
-Qed.
-
 Theorem eval_moduimm:
   forall le n a x z,
   eval_expr ge sp e m le a x ->
@@ -569,7 +527,7 @@ Proof.
   destruct (Int.is_power2 n) as []_eqn. 
   replace z with (Val.and x (Vint (Int.sub n Int.one))). apply eval_andimm; auto.
   eapply Val.modu_pow2; eauto.
-  exploit val_modu_divu; eauto. intros [v [A B]].
+  exploit Val.modu_divu; eauto. intros [v [A B]].
   subst. econstructor; split; eauto.
   apply eval_mod_aux with (semdivop := Val.divu); auto.
   EvalOp.
@@ -584,7 +542,7 @@ Theorem eval_modu:
 Proof.
   intros until y; unfold modu; case (modu_match b); intros; InvEval.
   eapply eval_moduimm; eauto.
-  exploit val_modu_divu; eauto. intros [v [A B]].
+  exploit Val.modu_divu; eauto. intros [v [A B]].
   subst. econstructor; split; eauto.
   apply eval_mod_aux with (semdivop := Val.divu); auto.
 Qed.
@@ -651,643 +609,260 @@ Proof.
   red; intros; TrivialExists.
 Qed.
 
-Inductive val_lessdef_upto: memory_chunk -> val -> val -> Prop :=
-  | val_lessdef_upto_undef: forall chunk v,
-      val_lessdef_upto chunk Vundef v
-  | val_lessdef_upto_int8: forall n1 n2,
-      Int.zero_ext 8 n1 = Int.zero_ext 8 n2 ->
-      val_lessdef_upto Mint8unsigned (Vint n1) (Vint n2)
-  | val_lessdef_upto_int16: forall n1 n2,
-      Int.zero_ext 16 n1 = Int.zero_ext 16 n2 ->
-      val_lessdef_upto Mint16unsigned (Vint n1) (Vint n2)
-  | val_lessdef_upto_float32: forall f1 f2,
-      Float.singleoffloat f1 = Float.singleoffloat f2 ->
-      val_lessdef_upto Mfloat32 (Vfloat f1) (Vfloat f2)
-  | val_lessdef_upto_refl: forall chunk v,
-      val_lessdef_upto chunk v v.
-
-Remark val_lessdef_upto_trans:
-  forall chunk v1 v2 v3, val_lessdef_upto chunk v1 v2 -> val_lessdef_upto chunk v2 v3 -> val_lessdef_upto chunk v1 v3.
-Proof.
-  intros. inv H.
-  constructor.
-  inv H0. constructor. congruence. constructor. auto.
-  inv H0. constructor. congruence. constructor. auto.
-  inv H0. constructor. congruence. constructor. auto.
-  auto.
-Qed.
-
-Lemma eval_uncast_int8:
-  forall le a x,
-  eval_expr ge sp e m le a x ->
-  exists v, eval_expr ge sp e m le (uncast_int8 a) v /\ val_lessdef_upto Mint8unsigned x v.
-Proof.
-  intros until a. functional induction (uncast_int8 a); intros.
-  (* cast8signed *)
-  InvEval. exploit IHe0; eauto. intros [v [A B]]. exists v; split; auto.
-  eapply val_lessdef_upto_trans; eauto. 
-  subst x. destruct v1; simpl; constructor. apply Int.zero_ext_sign_ext.
-  (* cast16signed *)
-  InvEval. exploit IHe0; eauto. intros [v [A B]]. exists v; split; auto.
-  eapply val_lessdef_upto_trans; eauto.
-  subst x. destruct v1; simpl; constructor. admit.
-  (* andimm *)
-  InvEval. exploit IHe0; eauto. intros [v [A B]]. exists v; split; auto.
-  eapply val_lessdef_upto_trans; eauto. 
-  subst. generalize (Int.eq_spec (Int.and n (Int.repr 255)) (Int.repr 255)); rewrite e2; intro EQ.
-  destruct v1; simpl; constructor. 
-  repeat rewrite Int.zero_ext_and. rewrite Int.and_assoc. decEq. assumption.
-  compute; auto. compute; auto.
-  exists x; split; auto. constructor.
-  (* default *)
-  exists x; split; auto. constructor.
-Qed.
-
-Lemma encode_val_lessdef_upto:
-  forall chunk v1 v2,
-  val_lessdef_upto chunk v1 v2 ->
-  list_forall2 (memval_inject inject_id) (encode_val chunk v1) (encode_val chunk v2).
-Proof.
-  induction 1.
-  (* undef *)
-  apply encode_val_inject. constructor.
-  (* two 8-bits ints *)
-  simpl. replace (encode_int Mint8unsigned n2) with (encode_int Mint8unsigned n1). 
-  apply inj_bytes_inject.
-  rewrite <- (encode_int8_zero_ext n1). 
-  rewrite <- (encode_int8_zero_ext n2).
-  congruence.
-  (* two 16-bits ints *)
-  simpl. replace (encode_int Mint16unsigned n2) with (encode_int Mint16unsigned n1). 
-  apply inj_bytes_inject.
-  rewrite <- (encode_int16_zero_ext n1). 
-  rewrite <- (encode_int16_zero_ext n2).
-  congruence.
-  (* two single floats *)
-  simpl. replace (encode_float Mfloat32 f2) with (encode_float Mfloat32 f1). 
-  apply inj_bytes_inject.
-  unfold encode_float. 
-  rewrite <- (Float.bits_of_singleoffloat f1).
-  rewrite <- (Float.bits_of_singleoffloat f2).
-  congruence.
-  (* same values *)
-  apply encode_val_inject. rewrite val_inject_id. auto.
-Qed.
-
-Lemma eval_uncast:
-  forall le chunk b ofs a x m1,
-  eval_expr ge sp e m le a x ->
-  Mem.store chunk m b ofs x = Some m1 ->
-  exists v, exists m2,
-     eval_expr ge sp e m le (uncast chunk a) v
-  /\ Mem.store chunk m b ofs v = Some m2
-  /\ Mem.extends m1 m2.
-Proof.
-  
-val_lessdef_upto Mint8unsigned x v.
-
-
-
-
-Inductive val_lessdef_int (n: Z): val -> val -> Prop :=
-  | val_lessdef_int_undef: forall v, val_lessdef_int n Vundef v
-  | val_lessdef_int_int: forall n1 n2, Int.zero_ext n n1 = Int.zero_ext n n2 -> val_lessdef_int n (Vint n1) (Vint n2)
-  | val_lessdef_int_refl: forall v, val_lessdef_int n v v.
-(*
-Definition val_lessdef_int_N (n: Z) (v1 v2: val): Prop :=
-  match v1, v2 with
-  | Vundef, _ => True
-  | Vint n1, Vint n2 => Int.zero_ext n n1 = Int.zero_ext n n2
-  | _, _ => v1 = v2
-  end.
-*)
-Remark val_lessdef_int_trans:
-  forall n v1 v2 v3, val_lessdef_int n v1 v2 -> val_lessdef_int n v2 v3 -> val_lessdef_int n v1 v3.
-Proof.
-  intros. inv H.
-  constructor.
-  inv H0. constructor. congruence. constructor. auto.
-  auto.
-Qed.
-
-Lemma eval_uncast_int8:
-  forall le a x,
-  eval_expr ge sp e m le a x ->
-  exists v, eval_expr ge sp e m le (uncast_int8 a) v /\ val_lessdef_int 8 x v.
-Proof.
-  intros until a. functional induction (uncast_int8 a); intros.
-  (* cast8signed *)
-  InvEval. exploit IHe0; eauto. intros [v [A B]]. exists v; split; auto.
-  eapply val_lessdef_int_trans; eauto. 
-  subst x. destruct v1; simpl; constructor. apply Int.zero_ext_sign_ext.
-  (* cast16signed *)
-  InvEval. exploit IHe0; eauto. intros [v [A B]]. exists v; split; auto.
-  eapply val_lessdef_int_trans; eauto.
-  subst x. destruct v1; simpl; constructor. admit.
-  (* andimm *)
-  InvEval. exploit IHe0; eauto. intros [v [A B]]. exists v; split; auto.
-  eapply val_lessdef_int_trans; eauto. 
-  subst. generalize (Int.eq_spec (Int.and n (Int.repr 255)) (Int.repr 255)); rewrite e2; intro EQ.
-  destruct v1; simpl; constructor. 
-  repeat rewrite Int.zero_ext_and. rewrite Int.and_assoc. decEq. assumption.
-  compute; auto. compute; auto.
-  exists x; split; auto. constructor.
-  (* default *)
-  exists x; split; auto. constructor.
-Qed.
-
-Remark memval_lessdef_trans:
-  forall v1 v2 v3, memval_lessdef v1 v2 -> memval_lessdef v2 v3 -> memval_lessdef v1 v3.
-Proof.
-  intros. inv H. auto. unfold inject_id in H1. inv H1. rewrite Int.add_zero in H0. auto. constructor.
-Qed.
-
-Definition memvals_lessdef (vl1 vl2: list memval) : Prop :=
-  list_forall2 memval_lessdef vl1 vl2.
-
-Remark memvals_lessdef_refl:
-  forall vl, memvals_lessdef vl vl.
-Proof.
-  induction vl; constructor; auto. apply memval_lessdef_refl.
-Qed.
-
-Remark memvals_lessdef_trans:
-  forall vl1 vl2, memvals_lessdef vl1 vl2 -> forall vl3, memvals_lessdef vl2 vl3 -> memvals_lessdef vl1 vl3.
-Proof.
-  induction 1; intros. inv H. constructor. 
-  inv H1. constructor. eapply memval_lessdef_trans; eauto. eapply IHlist_forall2; eauto.
-Qed.
-
-Remark memvals_lessdef_encode_val:
-  forall chunk v1 v2,
-  Val.lessdef v1 v2 ->
-  memvals_lessdef (encode_val chunk v1) (encode_val chunk v2).
-Proof.
-  intros. apply encode_val_inject. rewrite val_inject_id. auto.
-Qed.
-
-Lemma foo:
-  forall v1 v2,
-  val_lessdef_int 8 v1 v2 -> memvals_lessdef (encode_val Mint8unsigned v1) (encode_val Mint8unsigned v2).
-Proof.
-  induction 1.
-  (* undef *)
-  apply encode_val_inject. constructor.
-  (* two ints *)
-  simpl. replace (encode_int Mint8unsigned n2) with (encode_int Mint8unsigned n1). 
-  apply inj_bytes_inject.
-  rewrite <- (encode_int8_zero_ext n1). 
-  rewrite <- (encode_int8_zero_ext n2).
-  congruence.
-  (* same values *)
-  apply encode_val_inject. rewrite val_inject_id. auto.
-Qed.
-
-  replace (encode_val Mint8unsigned Vundef) with (list_repeat (List.length (encode_val Mint8unsigned v)) Undef).
-  apply repeat_U
-  simpl. 
-
-
-
-
-Lemma eval_uncast_int8:
-  forall le a x,
-  eval_expr ge sp e m le a x ->
-  exists v, eval_expr ge sp e m le (uncast_int8 a) v /\ 
-            memvals_lessdef (encode_val Mint8unsigned x) (encode_val Mint8unsigned v).
-Proof.
-  intros until a. functional induction (uncast_int8 a); intros.
-  (* cast8signed *)
-  InvEval. exploit IHe0; eauto. intros [v [A B]]. exists v; split; auto.
-  eapply memvals_lessdef_trans; eauto. subst x. 
-  destruct v1; simpl Val.sign_ext; try (apply memvals_lessdef_encode_val; auto; fail).
-  simpl. repeat rewrite <- encode_int8_signed_unsigned. 
-  rewrite encode_int8_sign_ext. apply memvals_lessdef_refl.
-  (* cast16signed *)
-  InvEval. exploit IHe0; eauto. intros [v [A B]]. exists v; split; auto.
-  eapply memvals_lessdef_trans; eauto. subst x. 
-  destruct v1; simpl Val.sign_ext; try (apply memvals_lessdef_encode_val; auto; fail).
-  simpl. repeat rewrite <- encode_int8_signed_unsigned. 
-  rewrite encode_int8_sign_ext. apply memvals_lessdef_refl.
-
-encode_change (encode_int Mint8unsrewrite encode_int8_sign_ext. 
-
- replace (encode_val Mint8unsigned x) with (encode_val Mint8unsigned v1). eauto.
-  subst. destruct v1; simpl Val.sign_ext. ; auto. rewrite Int.zero_ext_sign_ext; auto. 
-  (* cast16signed *)
-  InvEval. replace (Val.zero_ext 8 x) with (Val.zero_ext 8 v1). eauto. 
-  subst. destruct v1; simpl; auto. decEq. 
-  admit.
-  (* andimm *)
-  InvEval. replace (Val.zero_ext 8 x) with (Val.zero_ext 8 v1). eauto.
-  subst. generalize (Int.eq_spec (Int.and n (Int.repr 255)) (Int.repr 255)); rewrite e2; intro EQ.
-  destruct v1; simpl; auto. decEq. 
-  repeat rewrite Int.zero_ext_and. rewrite Int.and_assoc. decEq. symmetry. assumption.
-  compute; auto. compute; auto.
-  exists x; auto. 
-  (* default *)
-  exists x; auto.
-Qed.
-
-
-Lemma eval_uncast_int8:
-  forall le a x,
-  eval_expr ge sp e m le a x ->
-  exists v, eval_expr ge sp e m le (uncast_int8 a) v /\ Val.lessdef (Val.zero_ext 8 x) (Val.zero_ext 8 v).
-Proof.
-  intros until a. functional induction (uncast_int8 a); intros.
-  (* cast8signed *)
-  InvEval. replace (Val.zero_ext 8 x) with (Val.zero_ext 8 v1). eauto. 
-  subst. destruct v1; simpl; auto. rewrite Int.zero_ext_sign_ext; auto. 
-  (* cast16signed *)
-  InvEval. replace (Val.zero_ext 8 x) with (Val.zero_ext 8 v1). eauto. 
-  subst. destruct v1; simpl; auto. decEq. 
-  admit.
-  (* andimm *)
-  InvEval. replace (Val.zero_ext 8 x) with (Val.zero_ext 8 v1). eauto.
-  subst. generalize (Int.eq_spec (Int.and n (Int.repr 255)) (Int.repr 255)); rewrite e2; intro EQ.
-  destruct v1; simpl; auto. decEq. 
-  repeat rewrite Int.zero_ext_and. rewrite Int.and_assoc. decEq. symmetry. assumption.
-  compute; auto. compute; auto.
-  exists x; auto. 
-  (* default *)
-  exists x; auto.
-Qed.
-
-Lemma eval_uncast_int16:
-  forall le a x,
-  eval_expr ge sp e m le a x ->
-  exists v, eval_expr ge sp e m le (uncast_int16 a) v /\ Val.lessdef (Val.zero_ext 16 x) (Val.zero_ext 16 v).
-Proof.
-  intros until a. functional induction (uncast_int16 a); intros.
-  (* cast16signed *)
-  InvEval. replace (Val.zero_ext 16 x) with (Val.zero_ext 16 v1). eauto. 
-  subst. destruct v1; simpl; auto. rewrite Int.zero_ext_sign_ext; auto. 
-  (* andimm *)
-  InvEval. replace (Val.zero_ext 16 x) with (Val.zero_ext 16 v1). eauto.
-  subst. generalize (Int.eq_spec (Int.and n (Int.repr 65535)) (Int.repr 65535)); rewrite e2; intro EQ.
-  destruct v1; simpl; auto. decEq. 
-  repeat rewrite Int.zero_ext_and. rewrite Int.and_assoc. decEq. symmetry. assumption.
-  compute; auto. compute; auto.
-  exists x; auto. 
-  (* default *)
-  exists x; auto.
-Qed.
-
-Lemma eval_uncast_float32:
-  forall le a x,
-  eval_expr ge sp e m le a x ->
-  exists v, eval_expr ge sp e m le (uncast_float32 a) v /\ Val.lessdef (Val.singleoffloat x) (Val.singleoffloat v).
-Proof.
-  intros until a. functional induction (uncast_float32 a); intros.
-  (* cast16signed *)
-  InvEval. replace (Val.singleoffloat x) with (Val.singleoffloat v1). eauto. 
-  subst. destruct v1; simpl; auto. rewrite Float.singleoffloat_idem. auto.
-  (* default *)
-  exists x; auto.
-Qed.
-
-(* Move elsewhere *)
-
-Remark repeat_Undef_inject_encode_int:
-  forall f n chunk i,
-  size_chunk_nat chunk = n ->
-  list_forall2 (memval_inject f) (list_repeat n Undef) (inj_bytes (encode_int chunk i)).
-Proof.
-  intros. replace n with (List.length (inj_bytes (encode_int chunk i))).
-  apply repeat_Undef_inject_any. rewrite length_inj_bytes. rewrite encode_int_length. auto.
-Qed.
- 
-Remark repeat_Undef_inject_encode_float:
-  forall f n chunk i,
-  size_chunk_nat chunk = n ->
-  list_forall2 (memval_inject f) (list_repeat n Undef) (inj_bytes (encode_float chunk i)).
-Proof.
-  intros. replace n with (List.length (inj_bytes (encode_float chunk i))).
-  apply repeat_Undef_inject_any. rewrite length_inj_bytes. rewrite encode_float_length. auto.
-Qed.
-
-Remark val_inject_int:
-  forall f x y, val_inject f (Vint x) (Vint y) -> x = y.
-Proof.
-  intros. inv H; auto. 
-Qed.
-
-Remark val_inject_float:
-  forall f x y, val_inject f (Vfloat x) (Vfloat y) -> x = y.
-Proof.
-  intros. inv H; auto. 
-Qed.
-
-Ltac SolveIt :=
-  match goal with
-  | [ |- list_forall2 (memval_inject ?f) (Undef :: ?l) (Undef :: _) ] =>
-      exact (repeat_Undef_inject_self f (List.length (Undef :: l)))
-  | [ |- list_forall2 (memval_inject ?f) (Undef :: ?l) (inj_bytes (encode_int _ _)) ] =>
-      apply (repeat_Undef_inject_encode_int f (List.length (Undef :: l))); reflexivity
-  | [ |- list_forall2 (memval_inject ?f) (Undef :: ?l) (inj_bytes (encode_float _ _)) ] =>
-      apply (repeat_Undef_inject_encode_float f (List.length (Undef :: l))); reflexivity
-  | [ H: val_inject _ _ Vundef |- _ ] => inversion H
-  | [ H: val_inject _ (Vint _) (Vint _) |- _ ] => generalize (val_inject_int _ _ _ H); intro
-  | [ H: val_inject _ (Vfloat _) _ |- _ ] => generalize (val_inject_float _ _ _ H); intro
-  | _ => idtac
-  end.
-
-Lemma encode_val_inject_gen:
-  forall f chunk v1 v2,
-  val_inject f (Val.load_result chunk v1) (Val.load_result chunk v2) ->
-  list_forall2 (memval_inject f) (encode_val chunk v1) (encode_val chunk v2).
-Proof.
-  intros. unfold Val.load_result in H. destruct chunk; destruct v1; destruct v2; simpl; SolveIt.
-Focus 2.
-
-  inv H.
-Opaque Int.sign_ext. 
-  inv H. admit.
-
-
-; simpl in H; inv H.
-
-apply (repeat_Undef_inject_enco
-
-
-  repeat constructor.
-  
-
-
-  eapply repeat_Undef_inject_any. 
-  repeat constructor. 
-
-Lemma encode_val_load_result:
-  forall chunk v, encode_val chunk (Val.load_result chunk v) = encode_val chunk v.
-Proof.
-  intros. destruct chunk; destruct v; simpl; auto.
-Focus 2.
-  unfold encode_float. simpl. unfold rev_if_be. 
-
-Theorem eval_store_uncast:
-  forall chunk b ofs m' le a x,
-  eval_expr ge sp e m le a x ->
-  Mem.store chunk m b ofs x = Some m' ->
-  exists v, exists m'',
-     eval_expr ge sp e m le (uncast chunk a) v
-  /\ Mem.store chunk m b ofs v = Some m''
-  /\ Mem.extends m' m''.
-Proof.
-  intros. destruct chunk; simpl uncast.
-(* int8signed *)
-  exploit eval_uncast_int8; eauto. intros [v [A B]].
-  
-  
-
-
-
-
-  
-  rewrite Int.and_assoc. 
-  transitivity (Int.zero_ext 8 (Int.zero_ext 16 (Int.sign_ext 16 i))).
-  rewrite Int.zero_ext_widen. 
-
- rewrite Int.zero_ext_sign_ext; auto. 
-
-exploit IHe0; eauto. intros [v [A B]]. 
-  destruct e0. InvEval. destruct e1; InvEval. 
-  exploit 
-[idtac | InvEval ]. InvEval.  
-
-Theorem eval_cast8signed: unary_constructor_sound cast8signed (Val.sign_ext 8).
-
-Theorem eval_cast8unsigned: unary_constructor_sound cast8unsigned (Val.zero_ext 8).
-
-Theorem eval_cast16signed: unary_constructor_sound cast16signed (Val.sign_ext 16).
-
-Theorem eval_cast16unsigned: unary_constructor_sound cast16unsigned (Val.zero_ext 16).
-
-Theorem eval_singleoffloat: unary_constructor_sound singleoffloat Val.singleoffloat.
-
 Theorem eval_comp:
-  forall le c a x b y,
-  eval_expr ge sp e m le a (Vint x) ->
-  eval_expr ge sp e m le b (Vint y) ->
-  eval_expr ge sp e m le (comp c a b) (Val.of_bool(Int.cmp c x y)).
+  forall c, binary_constructor_sound (comp c) (Val.cmp c).
 Proof.
-  intros until y.
-  unfold comp; case (comp_match a b); intros; InvEval.
-  EvalOp. simpl. rewrite Int.swap_cmp. destruct (Int.cmp c x y); reflexivity.
-  EvalOp. simpl. destruct (Int.cmp c x y); reflexivity.
-  EvalOp. simpl. destruct (Int.cmp c x y); reflexivity.
+  intros; red; intros until y. unfold comp; case (comp_match a b); intros; InvEval.
+  TrivialExists. simpl. rewrite Val.swap_cmp_bool. auto.
+  TrivialExists.
+  TrivialExists.
 Qed.
 
-Theorem eval_compu_int:
-  forall le c a x b y,
-  eval_expr ge sp e m le a (Vint x) ->
-  eval_expr ge sp e m le b (Vint y) ->
-  eval_expr ge sp e m le (compu c a b) (Val.of_bool(Int.cmpu c x y)).
+Theorem eval_compu:
+  forall c, binary_constructor_sound (compu c) (Val.cmpu (Mem.valid_pointer m) c).
 Proof.
-  intros until y.
-  unfold compu; case (comp_match a b); intros; InvEval.
-  EvalOp. simpl. rewrite Int.swap_cmpu. destruct (Int.cmpu c x y); reflexivity.
-  EvalOp. simpl. destruct (Int.cmpu c x y); reflexivity.
-  EvalOp. simpl. destruct (Int.cmpu c x y); reflexivity.
-Qed.
-
-Remark eval_compare_null_transf:
-  forall c x v,
-  Cminor.eval_compare_null c x = Some v ->
-  match eval_compare_null c x with
-  | Some true => Some Vtrue
-  | Some false => Some Vfalse
-  | None => None (A:=val)
-  end = Some v.
-Proof.
-  unfold Cminor.eval_compare_null, eval_compare_null; intros.
-  destruct (Int.eq x Int.zero); try discriminate. 
-  destruct c; try discriminate; auto.
-Qed.
-
-Theorem eval_compu_ptr_int:
-  forall le c a x1 x2 b y v,
-  eval_expr ge sp e m le a (Vptr x1 x2) ->
-  eval_expr ge sp e m le b (Vint y) ->
-  Cminor.eval_compare_null c y = Some v ->
-  eval_expr ge sp e m le (compu c a b) v.
-Proof.
-  intros until v.
-  unfold compu; case (comp_match a b); intros; InvEval.
-  EvalOp. simpl. apply eval_compare_null_transf; auto.
-  EvalOp. simpl. apply eval_compare_null_transf; auto.
-Qed.
-
-Remark eval_compare_null_swap:
-  forall c x,
-  Cminor.eval_compare_null (swap_comparison c) x = 
-  Cminor.eval_compare_null c x.
-Proof.
-  intros. unfold Cminor.eval_compare_null. 
-  destruct (Int.eq x Int.zero). destruct c; auto. auto.
-Qed.
-
-Theorem eval_compu_int_ptr:
-  forall le c a x b y1 y2 v,
-  eval_expr ge sp e m le a (Vint x) ->
-  eval_expr ge sp e m le b (Vptr y1 y2) ->
-  Cminor.eval_compare_null c x = Some v ->
-  eval_expr ge sp e m le (compu c a b) v.
-Proof.
-  intros until v.
-  unfold compu; case (comp_match a b); intros; InvEval.
-  EvalOp. simpl. apply eval_compare_null_transf. 
-  rewrite eval_compare_null_swap; auto.
-  EvalOp. simpl. apply eval_compare_null_transf. auto.
-Qed.
-
-Theorem eval_compu_ptr_ptr:
-  forall le c a x1 x2 b y1 y2,
-  eval_expr ge sp e m le a (Vptr x1 x2) ->
-  eval_expr ge sp e m le b (Vptr y1 y2) ->
-  Mem.valid_pointer m x1 (Int.unsigned x2)
-  && Mem.valid_pointer m y1 (Int.unsigned y2) = true ->
-  x1 = y1 ->
-  eval_expr ge sp e m le (compu c a b) (Val.of_bool(Int.cmpu c x2 y2)).
-Proof.
-  intros until y2.
-  unfold compu; case (comp_match a b); intros; InvEval.
-  EvalOp. simpl. rewrite H1. subst y1. rewrite dec_eq_true. 
-  destruct (Int.cmpu c x2 y2); reflexivity.
-Qed.
-
-Theorem eval_compu_ptr_ptr_2:
-  forall le c a x1 x2 b y1 y2 v,
-  eval_expr ge sp e m le a (Vptr x1 x2) ->
-  eval_expr ge sp e m le b (Vptr y1 y2) ->
-  Mem.valid_pointer m x1 (Int.unsigned x2)
-  && Mem.valid_pointer m y1 (Int.unsigned y2) = true ->
-  x1 <> y1 ->
-  Cminor.eval_compare_mismatch c = Some v ->
-  eval_expr ge sp e m le (compu c a b) v.
-Proof.
-  intros until y2.
-  unfold compu; case (comp_match a b); intros; InvEval.
-  EvalOp. simpl. rewrite H1. rewrite dec_eq_false; auto.
-  destruct c; simpl in H3; inv H3; auto.
+  intros; red; intros until y. unfold compu; case (compu_match a b); intros; InvEval.
+  TrivialExists. simpl. rewrite Val.swap_cmpu_bool. auto.
+  TrivialExists.
+  TrivialExists.
 Qed.
 
 Theorem eval_compf:
-  forall le c a x b y,
-  eval_expr ge sp e m le a (Vfloat x) ->
-  eval_expr ge sp e m le b (Vfloat y) ->
-  eval_expr ge sp e m le (compf c a b) (Val.of_bool(Float.cmp c x y)).
+  forall c, binary_constructor_sound (compf c) (Val.cmpf c).
 Proof.
-  intros. unfold compf. EvalOp. simpl. 
-  destruct (Float.cmp c x y); reflexivity.
+  intros; red; intros. unfold compf. TrivialExists.
 Qed.
 
-Theorem eval_negint:
+Theorem eval_uncast_int8:
   forall le a x,
-  eval_expr ge sp e m le a (Vint x) ->
-  eval_expr ge sp e m le (negint a) (Vint (Int.neg x)).
-Proof. intros; unfold negint; EvalOp. Qed.
+  eval_expr ge sp e m le a x ->
+  exists v, eval_expr ge sp e m le (uncast_int8 a) v
+         /\ (Val.lessdef x v \/
+             exists p, exists q, x = Vint p /\ v = Vint q /\ Int.zero_ext 8 p = Int.zero_ext 8 q).
+Proof.
+  intros until a. functional induction (uncast_int8 a); intros.
+  (* cast8signed *)
+  InvEval. exploit IHe0; eauto. intros [v [A B]]. exists v; split; auto.
+  destruct B as [B | [p [q [C [D E]]]]].
+  inv B. destruct v; simpl; auto. right; do 2 econstructor. split. eauto. split. eauto. 
+  apply Int.zero_ext_sign_ext. 
+  simpl; auto.
+  subst. simpl. right; do 2 econstructor. split. eauto. split. eauto.
+  rewrite Int.zero_ext_sign_ext. auto.
+  (* cast16signed *)
+  InvEval. exploit IHe0; eauto. intros [v [A B]]. exists v; split; auto.
+  destruct B as [B | [p [q [C [D E]]]]].
+  inv B. destruct v; simpl; auto. right; do 2 econstructor. split. eauto. split. eauto. 
+  apply Int.zero_sign_ext_widen. compute; auto. split. omega. compute; auto.
+  simpl; auto.
+  subst. simpl. right; do 2 econstructor. split. eauto. split. eauto.
+  rewrite Int.zero_sign_ext_widen. auto. compute; auto. split. omega. compute; auto.
+  (* andimm *)
+  generalize (Int.eq_spec (Int.and n (Int.repr 255)) (Int.repr 255)); rewrite e2; intro EQ.
+  InvEval. exploit IHe0; eauto. intros [v [A B]]. exists v; split; auto.
+  destruct B as [B | [p [q [C [D E]]]]].
+  inv B. destruct v; simpl; auto. right; do 2 econstructor. split. eauto. split. eauto.
+  repeat rewrite Int.zero_ext_and. rewrite Int.and_assoc. decEq. assumption. compute; auto. compute; auto.
+  simpl; auto.
+  subst. simpl. right; do 2 econstructor. split. eauto. split. eauto.
+  rewrite <- E. 
+  repeat rewrite Int.zero_ext_and. rewrite Int.and_assoc. decEq. assumption. compute; auto. compute; auto.
+  exists x; split; auto.
+  (* default *)
+  exists x; split; auto.
+Qed.
 
-Theorem eval_negf:
+Theorem eval_uncast_int16:
   forall le a x,
-  eval_expr ge sp e m le a (Vfloat x) ->
-  eval_expr ge sp e m le (negf a) (Vfloat (Float.neg x)).
-Proof. intros; unfold negf; EvalOp. Qed.
+  eval_expr ge sp e m le a x ->
+  exists v, eval_expr ge sp e m le (uncast_int16 a) v
+         /\ (Val.lessdef x v \/
+             exists p, exists q, x = Vint p /\ v = Vint q /\ Int.zero_ext 16 p = Int.zero_ext 16 q).
+Proof.
+  intros until a. functional induction (uncast_int16 a); intros.
+  (* cast16signed *)
+  InvEval. exploit IHe0; eauto. intros [v [A B]]. exists v; split; auto.
+  destruct B as [B | [p [q [C [D E]]]]].
+  inv B. destruct v; simpl; auto. right; do 2 econstructor. split. eauto. split. eauto. 
+  apply Int.zero_ext_sign_ext. 
+  simpl; auto.
+  subst. simpl. right; do 2 econstructor. split. eauto. split. eauto.
+  rewrite Int.zero_ext_sign_ext. auto.
+  (* andimm *)
+  generalize (Int.eq_spec (Int.and n (Int.repr 65535)) (Int.repr 65535)); rewrite e2; intro EQ.
+  InvEval. exploit IHe0; eauto. intros [v [A B]]. exists v; split; auto.
+  destruct B as [B | [p [q [C [D E]]]]].
+  inv B. destruct v; simpl; auto. right; do 2 econstructor. split. eauto. split. eauto.
+  repeat rewrite Int.zero_ext_and. rewrite Int.and_assoc. decEq. assumption. compute; auto. compute; auto.
+  simpl; auto.
+  subst. simpl. right; do 2 econstructor. split. eauto. split. eauto.
+  rewrite <- E. 
+  repeat rewrite Int.zero_ext_and. rewrite Int.and_assoc. decEq. assumption. compute; auto. compute; auto.
+  exists x; split; auto.
+  (* default *)
+  exists x; split; auto.
+Qed.
 
-Theorem eval_absf:
+Theorem eval_uncast_float32:
   forall le a x,
-  eval_expr ge sp e m le a (Vfloat x) ->
-  eval_expr ge sp e m le (absf a) (Vfloat (Float.abs x)).
-Proof. intros; unfold absf; EvalOp. Qed.
+  eval_expr ge sp e m le a x ->
+  exists v, eval_expr ge sp e m le (uncast_float32 a) v
+         /\ (Val.lessdef x v \/
+             exists p, exists q, x = Vfloat p /\ v = Vfloat q /\ Float.singleoffloat p = Float.singleoffloat q).
+Proof.
+  intros until a. functional induction (uncast_float32 a); intros.
+  (* singleoffloat *)
+  InvEval. exploit IHe0; eauto. intros [v [A B]]. exists v; split; auto.
+  destruct B as [B | [p [q [C [D E]]]]].
+  inv B. destruct v; simpl; auto. right; do 2 econstructor. split. eauto. split. eauto. 
+  apply Float.singleoffloat_idem. 
+  simpl; auto.
+  subst. simpl. right; do 2 econstructor. split. eauto. split. eauto.
+  rewrite Float.singleoffloat_idem. auto.
+  (* default *)
+  exists x; split; auto.
+Qed.
+
+Theorem eval_cast8signed: unary_constructor_sound cast8signed (Val.sign_ext 8).
+Proof.
+  red; intros. unfold cast8signed. 
+  exploit eval_uncast_int8; eauto. intros [v [A B]].
+  exists (Val.sign_ext 8 v); split. EvalOp. 
+  destruct B as [B | [p [q [C [D E]]]]].
+  apply Val.sign_ext_lessdef; auto. 
+  subst. simpl. replace (Int.sign_ext 8 q) with (Int.sign_ext 8 p); auto.
+  apply Int.sign_ext_equal_if_zero_equal; auto. compute; auto.
+Qed.
+
+Theorem eval_cast8unsigned: unary_constructor_sound cast8unsigned (Val.zero_ext 8).
+Proof.
+  red; intros. unfold cast8unsigned. 
+  exploit eval_uncast_int8; eauto. intros [v [A B]].
+  exploit (eval_andimm (Int.repr 255)); eauto. intros [w [U V]].
+  exists w; split; auto. eapply Val.lessdef_trans. 2: eexact V. 
+  rewrite <- Val.cast8unsigned_and.
+  destruct B as [B | [p [q [C [D E]]]]].
+  apply Val.zero_ext_lessdef; auto. 
+  subst. simpl. rewrite E. auto.
+Qed.
+
+Theorem eval_cast16signed: unary_constructor_sound cast16signed (Val.sign_ext 16).
+Proof.
+  red; intros. unfold cast16signed. 
+  exploit eval_uncast_int16; eauto. intros [v [A B]].
+  exists (Val.sign_ext 16 v); split. EvalOp. 
+  destruct B as [B | [p [q [C [D E]]]]].
+  apply Val.sign_ext_lessdef; auto. 
+  subst. simpl. replace (Int.sign_ext 16 q) with (Int.sign_ext 16 p); auto.
+  apply Int.sign_ext_equal_if_zero_equal; auto. compute; auto.
+Qed.
+
+Theorem eval_cast16unsigned: unary_constructor_sound cast16unsigned (Val.zero_ext 16).
+Proof.
+  red; intros. unfold cast16unsigned. 
+  exploit eval_uncast_int16; eauto. intros [v [A B]].
+  exploit (eval_andimm (Int.repr 65535)); eauto. intros [w [U V]].
+  exists w; split; auto. eapply Val.lessdef_trans. 2: eexact V. 
+  rewrite <- Val.cast16unsigned_and.
+  destruct B as [B | [p [q [C [D E]]]]].
+  apply Val.zero_ext_lessdef; auto. 
+  subst. simpl. rewrite E. auto.
+Qed.
+
+Theorem eval_singleoffloat: unary_constructor_sound singleoffloat Val.singleoffloat.
+Proof.
+  red; intros. unfold singleoffloat. 
+  exploit eval_uncast_float32; eauto. intros [v [A B]].
+  exists (Val.singleoffloat v); split. EvalOp. 
+  destruct B as [B | [p [q [C [D E]]]]].
+  apply Val.singleoffloat_lessdef; auto. 
+  subst. simpl. rewrite E. auto.
+Qed.
 
 Theorem eval_intoffloat:
-  forall le a x n,
-  eval_expr ge sp e m le a (Vfloat x) ->
-  Float.intoffloat x = Some n ->
-  eval_expr ge sp e m le (intoffloat a) (Vint n).
+  forall le a x y,
+  eval_expr ge sp e m le a x ->
+  Val.intoffloat x = Some y ->
+  exists v, eval_expr ge sp e m le (intoffloat a) v /\ Val.lessdef y v.
 Proof.
-  intros; unfold intoffloat; EvalOp. simpl. rewrite H0; auto.
+  intros; unfold intoffloat. TrivialExists. 
 Qed.
 
 Theorem eval_intuoffloat:
-  forall le a x n,
-  eval_expr ge sp e m le a (Vfloat x) ->
-  Float.intuoffloat x = Some n ->
-  eval_expr ge sp e m le (intuoffloat a) (Vint n).
+  forall le a x y,
+  eval_expr ge sp e m le a x ->
+  Val.intuoffloat x = Some y ->
+  exists v, eval_expr ge sp e m le (intuoffloat a) v /\ Val.lessdef y v.
 Proof.
-  intros. unfold intuoffloat. 
-  econstructor. eauto. 
+  intros. destruct x; simpl in H0; try discriminate.
+  destruct (Float.intuoffloat f) as [n|]_eqn; simpl in H0; inv H0.
+  exists (Vint n); split; auto. unfold intuoffloat.
   set (im := Int.repr Int.half_modulus).
   set (fm := Float.floatofintu im).
-  assert (eval_expr ge sp e m (Vfloat x :: le) (Eletvar O) (Vfloat x)).
+  assert (eval_expr ge sp e m (Vfloat f :: le) (Eletvar O) (Vfloat f)).
     constructor. auto. 
-  apply eval_Econdition with (v1 := Float.cmp Clt x fm).
+  econstructor. eauto.
+  apply eval_Econdition with (v1 := Float.cmp Clt f fm).
   econstructor. constructor. eauto. constructor. EvalOp. simpl; eauto. constructor.
   simpl. auto.
-  caseEq (Float.cmp Clt x fm); intros.
+  destruct (Float.cmp Clt f fm) as []_eqn.
   exploit Float.intuoffloat_intoffloat_1; eauto. intro EQ.
   EvalOp. simpl. rewrite EQ; auto.
   exploit Float.intuoffloat_intoffloat_2; eauto. intro EQ.
-  replace n with (Int.add (Int.sub n Float.ox8000_0000) Float.ox8000_0000).
-  apply eval_addimm. eapply eval_intoffloat; eauto.
-  apply eval_subf; auto. EvalOp.
-  rewrite Int.sub_add_opp. rewrite Int.add_assoc. apply Int.add_zero. 
+  set (t1 := Eop (Ofloatconst (Float.floatofintu Float.ox8000_0000)) Enil).
+  set (t2 := subf (Eletvar 0) t1).
+  set (t3 := intoffloat t2).
+  exploit (eval_subf (Vfloat f :: le) (Eletvar 0) (Vfloat f) t1). 
+    auto. unfold t1; EvalOp. simpl; eauto. 
+  fold t2. intros [v2 [A2 B2]]. simpl in B2. inv B2. 
+  exploit (eval_addimm Float.ox8000_0000 (Vfloat f :: le) t3).
+    unfold t3. unfold intoffloat. EvalOp. simpl. rewrite EQ. simpl. eauto. 
+  intros [v4 [A4 B4]]. simpl in B4. inv B4. 
+  rewrite Int.sub_add_opp in A4. rewrite Int.add_assoc in A4. 
+  rewrite (Int.add_commut (Int.neg Float.ox8000_0000)) in A4. 
+  rewrite Int.add_neg_zero in A4. 
+  rewrite Int.add_zero in A4.
+  auto.
 Qed.
 
 Theorem eval_floatofint:
-  forall le a x,
-  eval_expr ge sp e m le a (Vint x) ->
-  eval_expr ge sp e m le (floatofint a) (Vfloat (Float.floatofint x)).
+  forall le a x y,
+  eval_expr ge sp e m le a x ->
+  Val.floatofint x = Some y ->
+  exists v, eval_expr ge sp e m le (floatofint a) v /\ Val.lessdef y v.
 Proof.
-  intros. unfold floatofint. rewrite Float.floatofint_from_words.
-  apply eval_subf.
-  EvalOp. constructor. EvalOp. simpl; eauto.
-  constructor. apply eval_addimm. eauto. constructor.
-  simpl. auto. 
-  EvalOp. 
+  intros. destruct x; simpl in H0; inv H0.
+  exists (Vfloat (Float.floatofint i)); split; auto.
+  unfold floatofint.
+  set (t1 := addimm Float.ox8000_0000 a).
+  set (t2 := Eop Ofloatofwords (Eop (Ointconst Float.ox4330_0000) Enil ::: t1 ::: Enil)).
+  set (t3 := Eop (Ofloatconst (Float.from_words Float.ox4330_0000 Float.ox8000_0000)) Enil).
+  exploit (eval_addimm Float.ox8000_0000 le a). eauto. fold t1. 
+  intros [v1 [A1 B1]]. simpl in B1. inv B1.
+  exploit (eval_subf le t2). 
+  unfold t2. EvalOp. constructor. EvalOp. simpl; eauto. constructor. eauto. constructor. 
+  unfold eval_operation. eauto. 
+  instantiate (2 := t3). unfold t3. EvalOp. simpl; eauto.
+  intros [v2 [A2 B2]]. simpl in B2. inv B2. rewrite Float.floatofint_from_words. auto.
 Qed.
 
 Theorem eval_floatofintu:
-  forall le a x,
-  eval_expr ge sp e m le a (Vint x) ->
-  eval_expr ge sp e m le (floatofintu a) (Vfloat (Float.floatofintu x)).
+  forall le a x y,
+  eval_expr ge sp e m le a x ->
+  Val.floatofintu x = Some y ->
+  exists v, eval_expr ge sp e m le (floatofintu a) v /\ Val.lessdef y v.
 Proof.
-  intros. unfold floatofintu. rewrite Float.floatofintu_from_words.
-  apply eval_subf.
-  EvalOp. constructor. EvalOp. simpl; eauto.
-  constructor. eauto. constructor.
-  simpl. auto. 
-  EvalOp. 
+  intros. destruct x; simpl in H0; inv H0.
+  exists (Vfloat (Float.floatofintu i)); split; auto.
+  unfold floatofintu.
+  set (t2 := Eop Ofloatofwords (Eop (Ointconst Float.ox4330_0000) Enil ::: a ::: Enil)).
+  set (t3 := Eop (Ofloatconst (Float.from_words Float.ox4330_0000 Int.zero)) Enil).
+  exploit (eval_subf le t2). 
+  unfold t2. EvalOp. constructor. EvalOp. simpl; eauto. constructor. eauto. constructor. 
+  unfold eval_operation. eauto. 
+  instantiate (2 := t3). unfold t3. EvalOp. simpl; eauto.
+  intros [v2 [A2 B2]]. simpl in B2. inv B2. rewrite Float.floatofintu_from_words. auto.
 Qed.
-
-Theorem eval_xor:
-  forall le a x b y,
-  eval_expr ge sp e m le a (Vint x) ->
-  eval_expr ge sp e m le b (Vint y) ->
-  eval_expr ge sp e m le (xor a b) (Vint (Int.xor x y)).
-Proof. intros; unfold xor; EvalOp. Qed.
-
-Theorem eval_shr:
-  forall le a x b y,
-  eval_expr ge sp e m le a (Vint x) ->
-  eval_expr ge sp e m le b (Vint y) ->
-  Int.ltu y Int.iwordsize = true ->
-  eval_expr ge sp e m le (shr a b) (Vint (Int.shr x y)).
-Proof. intros; unfold shr; EvalOp. simpl. rewrite H1. auto. Qed.
-
-Theorem eval_mulf:
-  forall le a x b y,
-  eval_expr ge sp e m le a (Vfloat x) ->
-  eval_expr ge sp e m le b (Vfloat y) ->
-  eval_expr ge sp e m le (mulf a b) (Vfloat (Float.mul x y)).
-Proof. intros; unfold mulf; EvalOp. Qed.
-
-Theorem eval_divf:
-  forall le a x b y,
-  eval_expr ge sp e m le a (Vfloat x) ->
-  eval_expr ge sp e m le b (Vfloat y) ->
-  eval_expr ge sp e m le (divf a b) (Vfloat (Float.div x y)).
-Proof. intros; unfold divf; EvalOp. Qed.
 
 Theorem eval_addressing:
   forall le chunk a v b ofs,
@@ -1302,18 +877,11 @@ Proof.
   intros until v. unfold addressing; case (addressing_match a); intros; InvEval.
   exists (@nil val). split. eauto with evalexpr. simpl. auto.
   exists (@nil val). split. eauto with evalexpr. simpl. auto.
-  destruct (Genv.find_symbol ge s); congruence.
-  exists (Vint i0 :: nil). split. eauto with evalexpr. 
-    simpl. destruct (Genv.find_symbol ge s). congruence. discriminate.
-  exists (Vptr b0 i :: nil). split. eauto with evalexpr. 
-    simpl. congruence.
-  exists (Vint i :: Vptr b0 i0 :: nil).
-    split. eauto with evalexpr. simpl. 
-    congruence.
-  exists (Vptr b0 i :: Vint i0 :: nil).
-    split. eauto with evalexpr. simpl. congruence.
-  exists (v :: nil). split. eauto with evalexpr. 
-    subst v. simpl. rewrite Int.add_zero. auto.
+  exists (v0 :: nil). split. eauto with evalexpr. simpl. congruence.
+  exists (v1 :: nil). split. eauto with evalexpr. simpl. congruence.
+  exists (v1 :: v0 :: nil). split. eauto with evalexpr. simpl. congruence.
+  exists (v :: nil). split. eauto with evalexpr. subst v. simpl. 
+  rewrite Int.add_zero. auto.
 Qed.
 
 End CMCONSTR.
